Fixed up HOL-UTP-THY so it builds again.

theories/theories/utp_acp.thy
@@ -14,16 +14,16 @@ imports
 begin
 
 definition ACP1 :: "'a WF_PREDICATE \<Rightarrow> 'a WF_PREDICATE" where
-"ACP1 P = `P \<and> (ok \<and> ($tr\<acute> = $tr) \<Rightarrow> $wait\<acute>)` "
+"ACP1 P = `P \<and> (($tr\<acute> = $tr) \<Rightarrow> $wait\<acute>)` "
 
 definition \<delta> :: "'a WF_PREDICATE" where
 "\<delta> = `R3($tr\<acute> =$tr \<and> $wait\<acute>)`"
 
-definition B :: "'a WF_PREDICATE" where
-"B = `($tr\<acute> = $tr \<and> $wait\<acute>) \<or> ($tr < $tr\<acute>)`"
+definition B_pred :: "'a WF_PREDICATE" where
+"B_pred = `($tr\<acute> = $tr \<and> $wait\<acute>) \<or> ($tr < $tr\<acute>)`"
 
 definition \<Phi> :: "'a WF_PREDICATE \<Rightarrow> 'a WF_PREDICATE" where
-"\<Phi>(P) = `RH(B \<and> P)`"
+"\<Phi>(P) = `RH(B_pred \<and> P)`"
 
 definition doA :: "('m EVENT, 'm) WF_PEXPRESSION \<Rightarrow> 'm WF_PREDICATE" where
 "doA(a) = `\<Phi>(a \<notin> $ref\<acute> \<lhd> $wait\<acute> \<rhd> ($tr^\<langle>a\<rangle> =$tr\<acute>))`"
@@ -31,12 +31,12 @@ definition doA :: "('m EVENT, 'm) WF_PEXPRESSION \<Rightarrow> 'm WF_PREDICATE" 
 definition alternative :: "'a WF_PREDICATE \<Rightarrow> 'a WF_PREDICATE \<Rightarrow> 'a WF_PREDICATE" ("_ +\<^bsub>ACP\<^esub> _") where
 "(P +\<^bsub>ACP\<^esub> Q) = `(P \<and> Q) \<lhd> \<delta> \<rhd> (P \<or> Q)`"
 
-declare ACP1_def [eval,evalr,evalrx]
-declare \<delta>_def [eval,evalr,evalrx]
-declare B_def [eval,evalr,evalrx]
-declare \<Phi>_def [eval,evalr,evalrx]
-declare doA_def [eval,evalr,evalrx]
-declare alternative_def [eval,evalr,evalrx]
+declare ACP1_def [eval,evalr,evalrx,evalp]
+declare \<delta>_def [eval,evalr,evalrx,evalp]
+declare B_pred_def [eval,evalr,evalrx,evalp]
+declare \<Phi>_def [eval,evalr,evalrx,evalp]
+declare doA_def [eval,evalr,evalrx,evalp]
+declare alternative_def [eval,evalr,evalrx,evalp]
 
 syntax 
   "_upred_doA" :: "uexpr \<Rightarrow> upred" ("do\<A>'(_')")
@@ -49,7 +49,7 @@ translations
 declare \<delta>_def [eval, evalr, evalrr, evalrx]
 declare doA_def [eval, evalr, evalrr, evalrx]
 declare \<Phi>_def [eval, evalr, evalrr, evalrx]
-declare B_def [eval, evalr, evalrr, evalrx]
+declare B_pred_def [eval, evalr, evalrr, evalrx]
 
 subsection {* Closure Laws *}
 
@@ -65,8 +65,8 @@ lemma \<delta>_rel_closure [closure]:
   done
 
 lemma B_rel_closure [closure]:
-  "`B` \<in> WF_RELATION"
-  by (simp add:B_def closure typing defined unrest WF_RELATION_UNREST)
+  "`B_pred` \<in> WF_RELATION"
+  by (simp add:B_pred_def closure typing defined unrest WF_RELATION_UNREST)
 
 lemma \<Phi>_rel_closure [closure]:
   "P \<in> WF_RELATION \<Longrightarrow> `\<Phi>(P)` \<in> WF_RELATION"
@@ -95,47 +95,34 @@ lemma ACP1_R1_commute:
 
 lemma ACP1_R2_commute: "ACP1(R2(P)) = R2(ACP1(P))" 
 proof -
-  have "R2(ACP1(P)) = `R2(P) \<and> (ok \<and> \<langle>\<rangle> = ($tr\<acute> - $tr) \<Rightarrow> $wait\<acute>)`"
-    by (simp add:ACP1_def R2_def R2s_def usubst typing defined closure, utp_pred_auto_tac)
+  have "R2(ACP1(P)) = `R2(P) \<and> (\<langle>\<rangle> = ($tr\<acute> - $tr) \<Rightarrow> $wait\<acute>)`"
+    apply (simp add:ACP1_def R2_def R2s_def usubst typing defined closure)
+    apply (utp_pred_auto_tac)
+    done
 
-  also have "... = `R2(P) \<and> ($tr \<le> $tr\<acute>) \<and> (ok \<and> \<langle>\<rangle> = ($tr\<acute> - $tr) \<Rightarrow> $wait\<acute>)`"
+  also have "... = `R2(P) \<and> ($tr \<le> $tr\<acute>) \<and> (\<langle>\<rangle> = ($tr\<acute> - $tr) \<Rightarrow> $wait\<acute>)`"
     by (smt AndP_assoc AndP_idem R1_def R2_def)
 
-  also have "... = `R2(P) \<and> ($tr \<le> $tr\<acute>) \<and> (($tr \<le> $tr\<acute>) \<and> ok \<and> \<langle>\<rangle> = ($tr\<acute> - $tr) \<Rightarrow> $wait\<acute>)`"
+  also have "... = `R2(P) \<and> ($tr \<le> $tr\<acute>) \<and> (($tr \<le> $tr\<acute>) \<and> \<langle>\<rangle> = ($tr\<acute> - $tr) \<Rightarrow> $wait\<acute>)`"
     by (metis (hide_lams, no_types) ImpliesP_AndP_pre)
 
-  also have "... = `R2(P) \<and> (($tr \<le> $tr\<acute>) \<and> ok \<and> \<langle>\<rangle> = ($tr\<acute> - $tr) \<Rightarrow> $wait\<acute>)`"
+  also have "... = `R2(P) \<and> (($tr \<le> $tr\<acute>) \<and> \<langle>\<rangle> = ($tr\<acute> - $tr) \<Rightarrow> $wait\<acute>)`"
     by (smt AndP_assoc AndP_idem R1_def R2_def)
 
-  also have "... = `R2(P) \<and> (ok \<and> \<langle>\<rangle> = ($tr\<acute> - $tr) \<and> ($tr \<le> $tr\<acute>) \<Rightarrow> $wait\<acute>)`"
+  also have "... = `R2(P) \<and> (\<langle>\<rangle> = ($tr\<acute> - $tr) \<and> ($tr \<le> $tr\<acute>) \<Rightarrow> $wait\<acute>)`"
     by (smt AndP_assoc AndP_comm)
 
-  also have "... = `R2(P) \<and> (ok \<and> ($tr\<acute> = $tr) \<Rightarrow> $wait\<acute>)`"
+  also have "... = `R2(P) \<and> (($tr\<acute> = $tr) \<Rightarrow> $wait\<acute>)`"
     by (metis (hide_lams, no_types) EqualP_sym tr_prefix_as_nil)
 
   finally show ?thesis 
     by (simp add:ACP1_def) 
 qed
 
-lemma ACP1_R3_commute: "ACP1 (R3 P) = R3 (ACP1 P)" 
-proof -
-  have "ACP1 (R3 P) = `($wait \<and> \<not> ok \<and> ($tr \<le> $tr\<acute>)) \<or> (ok' \<and> $wait \<and> II\<^bsub>REL_VAR - {okay\<down>, okay\<down>\<acute>}\<^esub> \<and> ( ok \<and> ($tr\<acute> =$tr) \<Rightarrow> $wait\<acute>)) \<or> (\<not>$wait \<and> P \<and> (ok \<and> ($tr\<acute> =$tr) \<Rightarrow> $wait\<acute>))`" 
-    by (simp add:ACP1_def R3_def SkipREA_def CondR_def, utp_pred_auto_tac)
-
-  also have "... = `($wait \<and> \<not> ok \<and> ($tr \<le> $tr\<acute>)) \<or> (ok' \<and> $wait \<and> $wait\<acute> \<and> II\<^bsub>REL_VAR - {okay\<down>, okay\<down>\<acute>}\<^esub> \<and> ( ok \<and> ($tr\<acute> =$tr) \<Rightarrow> $wait\<acute>)) \<or> (\<not>$wait \<and> P \<and> ( ok \<and> ($tr\<acute> =$tr) \<Rightarrow> $wait\<acute>))`" 
-    sorry
-
-  also have "... = `($wait \<and> \<not> ok \<and> ($tr \<le> $tr\<acute>)) \<or> (ok' \<and> $wait \<and> $wait\<acute> \<and> II\<^bsub>REL_VAR - {okay\<down>, okay\<down>\<acute>}\<^esub>) \<or> (\<not>$wait \<and> P \<and> ( ok \<and> ($tr\<acute> =$tr) \<Rightarrow> $wait\<acute>))`" 
-    by (utp_pred_auto_tac)
-
-  also have "... = `($wait \<and> \<not> ok \<and> ($tr \<le> $tr\<acute>)) \<or> (ok' \<and> $wait \<and> II\<^bsub>REL_VAR - {okay\<down>, okay\<down>\<acute>}\<^esub>) \<or> (\<not>$wait \<and> P \<and> ( ok \<and> ($tr\<acute> =$tr) \<Rightarrow> $wait\<acute>))`" 
-    sorry
-
-  also have "... = `R3(P \<and> ( ok \<and> ($tr\<acute> =$tr) \<Rightarrow> $wait\<acute>))`" 
-    by(simp add: R3_def CondR_def SkipREA_def, utp_pred_auto_tac)
-
-  finally show ?thesis by(simp add:ACP1_def)
-qed
+lemma ACP1_R3_commute: "ACP1 (R3 P) = R3 (ACP1 P)"
+  apply (utp_poly_auto_tac)
+  apply (simp add:closure Rep_binding_ty_def EvalP_SkipR)
+done
 
 lemma ACP1_OrP:
   "`ACP1(P \<or> Q)` = `ACP1(P) \<or> ACP1(Q)`"
@@ -149,16 +136,16 @@ lemma ACP1_CondR:
   "`ACP1(P \<lhd> b \<rhd> Q)` = `ACP1(P) \<lhd> ACP1(b) \<rhd> ACP1(Q)`"
   by (utp_pred_auto_tac)
 
-subsection {* \<delta> laws *}
+subsection {* Delta laws *}
 
 lemma R1_\<delta> : "`R1(\<delta>)` = `\<delta>`"
 proof -
-  have "`R1(\<delta>)`  = `(II\<^bsub>rea\<^esub> \<and> ($tr \<le> $tr\<acute>)) \<lhd> $wait \<rhd> ($tr =$tr\<acute> \<and> $wait\<acute> \<and> ($tr \<le> $tr\<acute>))`" 
+  have "`R1(\<delta>)`  = `(II \<and> ($tr \<le> $tr\<acute>)) \<lhd> $wait \<rhd> ($tr =$tr\<acute> \<and> $wait\<acute> \<and> ($tr \<le> $tr\<acute>))`" 
     by (simp add:\<delta>_def, utp_pred_auto_tac)
-  also have "... = `R1(II\<^bsub>rea\<^esub>) \<lhd> $wait \<rhd> ($tr\<acute> =$tr \<and> $wait\<acute> )`" 
-    by (utp_pred_auto_tac)
+  also have "... = `R1(II) \<lhd> $wait \<rhd> ($tr\<acute> =$tr \<and> $wait\<acute> )`" 
+    by utp_poly_auto_tac
   finally show ?thesis 
-    by (metis SkipREA_is_R1 R3_def \<delta>_def)
+    by (metis R1_SkipR R3_def \<delta>_def)
 qed
 
 lemma R2_\<delta> : "`R2(\<delta>)` = `\<delta>`" 
@@ -179,9 +166,9 @@ lemma R3_\<delta>: "`R3(\<delta>)` = `\<delta>`"
 lemma ACP1_\<delta>: "ACP1(\<delta>) = \<delta>" 
   by (simp add:is_healthy_def \<delta>_def ACP1_R3_commute, simp add:ACP1_def, utp_pred_auto_tac)
 
-lemma \<delta>_form: "\<delta> = `(\<not> ok \<and> $wait \<and> ($tr \<le> $tr\<acute>)) \<or> (ok \<and> $wait \<and> II) \<or> (\<not>$wait \<and> ($tr\<acute> = $tr) \<and> $wait\<acute>)`"
+lemma \<delta>_form: "\<delta> = `($wait \<and> II) \<or> (\<not>$wait \<and> ($tr\<acute> = $tr) \<and> $wait\<acute>)`"
   by(simp add: \<delta>_def R3_form) 
-
+  
 subsection {* doA laws *}
 
 lemma doA_is_R1: "`R1(do\<A>(a))` = `do\<A>(a)`"
@@ -195,38 +182,40 @@ lemma doA_is_R3: "`R3(do\<A>(a))` = `do\<A>(a)`"
 
 lemma doA_is_ACP1: "`do\<A>(a)` is ACP1" 
 proof -
-  have "`ACP1(B \<and>( a \<notin> $ref\<acute> \<lhd> $wait\<acute> \<rhd> ($tr^\<langle>a\<rangle> =$tr\<acute>)))` = `(B \<and>( a \<notin> $ref\<acute> \<lhd> $wait\<acute> \<rhd> ($tr^\<langle>a\<rangle> =$tr\<acute>)))`" 
-    by (simp add:ACP1_def CondR_def, utp_pred_auto_tac)
-  moreover have "`ACP1(do\<A>(a))` = `RH(ACP1(B \<and>( a \<notin> $ref\<acute> \<lhd> $wait\<acute> \<rhd> ($tr^\<langle>a\<rangle> =$tr\<acute>))))`" 
+  have "`ACP1(B_pred \<and>( a \<notin> $ref\<acute> \<lhd> $wait\<acute> \<rhd> ($tr^\<langle>a\<rangle> =$tr\<acute>)))` = `(B_pred \<and>( a \<notin> $ref\<acute> \<lhd> $wait\<acute> \<rhd> ($tr^\<langle>a\<rangle> =$tr\<acute>)))`" 
+    apply (simp add:ACP1_def CondR_def)
+    apply (utp_poly_auto_tac)
+    done
+  moreover have "`ACP1(do\<A>(a))` = `RH(ACP1(B_pred \<and>( a \<notin> $ref\<acute> \<lhd> $wait\<acute> \<rhd> ($tr^\<langle>a\<rangle> =$tr\<acute>))))`" 
     by (simp add:doA_def \<Phi>_def RH_def ACP1_R1_commute ACP1_R2_commute ACP1_R3_commute)
   ultimately show ?thesis by(simp add:is_healthy_def doA_def \<Phi>_def)
 qed
 
-lemma B_form: "B = `R1($wait\<acute> \<or> ($tr < $tr\<acute>))`"
-  apply (utp_pred_auto_tac)
-  apply (metis prefixI)
+lemma B_form: "B_pred = `R1($wait\<acute> \<or> ($tr < $tr\<acute>))`"
+  apply(utp_poly_auto_tac)
+  apply(metis prefixI)
 done
 
 lemma doA_form: 
   assumes "TR \<sharp> a"
   shows "`do\<A>(a)` = `R3(((a \<notin> $ref\<acute>) \<and> ($tr \<le> $tr\<acute>)) \<lhd> $wait\<acute> \<rhd> ($tr ^ \<langle>a\<rangle> = $tr\<acute>))`"
 proof -
-  have "`do\<A>(a)` = `RH(B \<and> ((a \<notin> $ref\<acute>) \<lhd> $wait\<acute> \<rhd> ($tr ^ \<langle>a\<rangle> = $tr\<acute>)))`" 
+  have "`do\<A>(a)` = `RH(B_pred \<and> ((a \<notin> $ref\<acute>) \<lhd> $wait\<acute> \<rhd> ($tr ^ \<langle>a\<rangle> = $tr\<acute>)))`" 
     by (simp add: doA_def \<Phi>_def)
 
   also have "... = `RH(((a \<notin> $ref\<acute>) \<and> ($tr \<le> $tr\<acute>)) \<lhd> $wait\<acute> \<rhd> (($tr ^ \<langle>a\<rangle> = $tr\<acute>) \<and> ($tr < $tr\<acute>)))`" 
     proof -
       have 1: "`($tr \<le> $tr\<acute>)` = `($tr < $tr\<acute>) \<or> ($tr\<acute> =  $tr)`"
-        by(utp_pred_auto_tac)
-      have 2: "`B \<and> $wait\<acute>` = `($tr \<le> $tr\<acute>) \<and> $wait\<acute>`"
-        apply(simp add:B_def "1")
+        by(utp_poly_auto_tac)
+      have 2: "`B_pred \<and> $wait\<acute>` = `($tr \<le> $tr\<acute>) \<and> $wait\<acute>`"
+        apply(simp add:B_pred_def "1")
         apply(utp_pred_auto_tac)
         done
-      have 3: "`B \<and> \<not>$wait\<acute>` = `($tr < $tr\<acute>) \<and> \<not>$wait\<acute>`"
-        apply(simp add:B_def)
+      have 3: "`B_pred \<and> \<not>$wait\<acute>` = `($tr < $tr\<acute>) \<and> \<not>$wait\<acute>`"
+        apply(simp add:B_pred_def)
         apply(utp_pred_auto_tac)
         done
-      have "`B \<and> ((a \<notin> $ref\<acute>) \<lhd> $wait\<acute> \<rhd> ($tr ^ \<langle>a\<rangle> = $tr\<acute>))` = `(B \<and> $wait\<acute> \<and> (a \<notin> $ref\<acute>)) \<or> (B \<and> \<not>$wait\<acute> \<and> ($tr ^ \<langle>a\<rangle> = $tr\<acute>))`"
+      have "`B_pred \<and> ((a \<notin> $ref\<acute>) \<lhd> $wait\<acute> \<rhd> ($tr ^ \<langle>a\<rangle> = $tr\<acute>))` = `(B_pred \<and> $wait\<acute> \<and> (a \<notin> $ref\<acute>)) \<or> (B_pred \<and> \<not>$wait\<acute> \<and> ($tr ^ \<langle>a\<rangle> = $tr\<acute>))`"
         apply(simp add:CondR_def)
         apply(utp_pred_auto_tac)
         done
@@ -245,7 +234,7 @@ proof -
   also from assms have "... = `R3(R1((a \<notin> $ref\<acute>) \<lhd> $wait\<acute> \<rhd> (\<langle>a\<rangle> = ($tr\<acute> - $tr))))`"
   proof -
     have "`(($tr ^ \<langle>a\<rangle> = $tr\<acute>) \<and> ($tr < $tr\<acute>))` = `($tr ^ \<langle>a\<rangle> = $tr\<acute>)`"
-      apply (utp_pred_auto_tac)
+      apply (utp_poly_auto_tac)
       apply (metis prefixI')
     done
 
@@ -264,10 +253,9 @@ proof -
   also from assms have "... = `R3(R1((a \<notin> $ref\<acute>) \<lhd> $wait\<acute> \<rhd> ($tr ^ \<langle>a\<rangle> = $tr\<acute>)))`"
   proof -
     have "`\<langle>a\<rangle> = ($tr\<acute> - $tr) \<and> ($tr \<le> $tr\<acute>)` = `($tr ^ \<langle>a\<rangle>) = $tr\<acute> \<and> ($tr \<le> $tr\<acute>)`"
-      apply (utp_pred_tac)
+      apply (utp_poly_tac)
       apply (rule)
       apply (subgoal_tac "set (drop (length (DestList (\<langle>b\<rangle>\<^sub>b tr\<down>))) (DestList (\<langle>b\<rangle>\<^sub>b tr\<down>\<acute>))) \<subseteq> dcarrier (EventType :: 'a UTYPE)")
-      apply (simp add:typing defined closure)
       apply (smt drop_Cons' drop_all drop_append prefixeq_drop self_append_conv2)
       apply (rule subset_trans, rule set_drop_subset, rule DestList_tr'_dcarrier)
     done
@@ -333,21 +321,14 @@ lemma L1 :
 proof -
   have 1: "`\<delta> ; P` is R3"
     apply(subst R3_SemiR_closure)
-    apply (metis \<delta>_rel_closure)
-    apply (metis assms(3))
-    apply (metis Healthy_intro R3_\<delta>)
-    apply (metis RH_is_R3 assms(2))
-    apply (metis RH_is_R1 assms(2))
-    apply (simp)
+    apply(simp_all add:\<delta>_rel_closure assms(3) Healthy_intro R3_\<delta> assms(2) RH_is_R3)
     done
   have 2: "`\<not>$wait \<and> \<delta>` = `\<not>$wait \<and> ($tr\<acute> = $tr) \<and> $wait\<acute>`" 
     by(utp_pred_auto_tac)
   have "`\<not>$wait \<and> \<delta>;P` = `(\<not>$wait \<and> \<delta>) ; P`"
     apply(subst SemiR_AndP_left_precond)
-    apply (metis \<delta>_rel_closure)
-    apply (metis assms(3))
+    apply(simp_all add:\<delta>_rel_closure assms(3))
     apply (utp_pred_auto_tac)
-    apply (simp)
     done
   also have "... = `(\<not>$wait \<and> ($tr\<acute> = $tr) \<and> $wait\<acute>) ; P`" 
     by(subst 2,simp)
@@ -364,94 +345,29 @@ proof -
 done
  also have "... = `(\<not>$wait \<and> ($tr\<acute> = $tr)) ; ($wait \<and> R3(P))`"
     by(metis assms(2) RH_is_R3 is_healthy_def)
-  also have "... = `(\<not>$wait \<and> ($tr\<acute> = $tr)) ; ($wait \<and> II\<^bsub>rea\<^esub>)`"
+  also have "... = `(\<not>$wait \<and> ($tr\<acute> = $tr)) ; ($wait \<and> II)`"
     by (metis AndP_comm R3_wait)
-  also have "... = `(\<not>$wait \<and> ($tr\<acute> = $tr) \<and> $wait\<acute>) ; II\<^bsub>rea\<^esub>`"
+  also have "... = `\<not>$wait \<and> ($tr\<acute> = $tr) \<and> $wait\<acute>`"
     apply(subst SemiR_AndP_right_precond)
     apply(subst AndP_rel_closure)
-    apply(utp_pred_auto_tac)
+    apply(simp_all add:closure urename)
     apply(metis tr_eq_rel_closure)
-    apply(simp_all)
-    apply(metis SkipREA_rel_closure)
-    apply(utp_pred_auto_tac)
-    apply(simp add: urename closure typing defined )
-by (metis (hide_lams, mono_tags) AndP_assoc)
-  also have "... = `\<not>$wait \<and> (($tr\<acute> = $tr) \<and> $wait\<acute>) ; II\<^bsub>rea\<^esub>`"
-    apply(subst SemiR_AndP_left_precond)
-    apply(subst AndP_rel_closure)
-    apply(metis tr_eq_rel_closure)
-    apply(utp_pred_auto_tac)
-    apply(simp_all)
-    apply(metis SkipREA_rel_closure)
-    apply(utp_pred_auto_tac)
+    apply(subst AndP_assoc, simp)
     done
-  finally have 3: "`\<not>$wait \<and> \<delta>;P` = `\<not>$wait \<and> (($tr\<acute> = $tr) \<and> $wait\<acute>) ; II\<^bsub>rea\<^esub>`"
+  finally have 3: "`\<not>$wait \<and> \<delta>;P` = `\<not>$wait \<and> ($tr\<acute> = $tr) \<and> $wait\<acute>`"
     ..
-  have "`(($tr\<acute> = $tr) \<and> $wait\<acute>) ; II\<^bsub>rea\<^esub>` = `
-        (($tr\<acute> = $tr) \<and> $wait\<acute>) ; (ok \<and> II\<^bsub>REL_VAR\<^esub>) \<or>
-        (($tr\<acute> = $tr) \<and> $wait\<acute>) ; (\<not>ok \<and> ($tr \<le> $tr\<acute>))`" 
-    by(simp add:SkipREA_CondR_SkipR CondR_def SemiR_OrP_distl SkipR_as_SkipRA)
-  also have "... = `
-        (($tr\<acute> = $tr) \<and> $wait\<acute> \<and> ok') ; II\<^bsub>REL_VAR\<^esub> \<or>
-        (($tr\<acute> = $tr) \<and> $wait\<acute> \<and> \<not>ok') ; ($tr \<le> $tr\<acute>)`"
-    apply(subst SemiR_AndP_right_precond)
-    apply(subst AndP_rel_closure)
-    apply(metis tr_eq_rel_closure)
-    apply(utp_pred_auto_tac)
-    apply(simp_all)
-    apply (metis SkipR_as_SkipRA SkipR_closure)
-    apply(utp_pred_auto_tac)
-    apply(subst SemiR_AndP_right_precond)
-    apply(subst AndP_rel_closure)
-    apply(metis tr_eq_rel_closure)
-    apply(utp_pred_auto_tac)
-    apply(simp_all)
-    apply (smt R1_def R1_rel_closure TrueP_rel_closure utp_pred_simps(6))
-    apply(utp_pred_auto_tac)    
-    apply(simp add: urename closure typing defined )
-    by (metis (hide_lams, no_types) AndP_assoc AndP_comm SemiR_assoc SkipR_as_SkipRA demorgan3 utp_pred_simps(15))
-  also have "... = `
-        (($tr\<acute> = $tr) \<and> $wait\<acute> \<and> ok')  \<or>
-        (($tr\<acute> = $tr) \<and> $wait\<acute> \<and> \<not>ok') ; ($tr \<le> $tr\<acute>)`"
-    apply(subst SkipRA_right_unit)
-    apply(subst AndP_rel_closure)
-    apply (metis tr_eq_rel_closure)
-    apply(utp_pred_auto_tac)
-    apply(simp_all add:closure unrest typing)
-    done
-  also have "... = `
-        (($tr\<acute> = $tr) \<and> $wait\<acute> \<and> ok')  \<or>
-        ($tr\<acute> = $tr) ; ((\<not>ok \<and> $wait) \<and> ($tr \<le> $tr\<acute>))`"
-    apply(subst SemiR_AndP_right_precond)
-    apply(simp_all add:closure typing WF_RELATION_UNREST defined unrest urename AndP_comm)
-    done
-  also have "... = `(($tr\<acute> = $tr) \<and> $wait\<acute> \<and> ok')  \<or> 
-                      ($tr\<acute> = $tr) ; ($tr \<le> $tr\<acute>)`"
-    apply(subst SemiR_remove_middle_unrest1[of "`($tr \<acute>=$tr)`" "`($tr \<le> $tr \<acute>)`" "{wait \<down>,okay \<down>}" "`\<not>ok \<and> $wait`"])
-    apply(simp_all add:closure unrest typing defined WF_RELATION_UNREST)
-    apply(utp_pred_auto_tac)
-    apply(rule_tac x="\<B>(okay\<down> :=\<^sub>b FalseV, wait\<down> :=\<^sub>b TrueV)" in exI)
-    apply(simp add:typing defined)
-  done
-  also have "... = `(($tr\<acute> = $tr) \<and> $wait\<acute> \<and> ok')  \<or> ($tr \<le> $tr\<acute>)`"
-    by (metis tr_eq_tr_leq)
-  finally have 4: "`(($tr\<acute> = $tr) \<and> $wait\<acute>) ; II\<^bsub>rea\<^esub>` = `($tr \<le> $tr\<acute>)`"
-    by(utp_pred_auto_tac)
   have "`\<delta> ; P` = `R3(\<delta> ; P)`"
     by(metis "1" is_healthy_def)
-  also have "... = `(\<not>ok \<and> $wait \<and> ($tr \<le> $tr\<acute>)) \<or> (ok \<and> $wait \<and> II) \<or> (\<not>$wait \<and> \<delta> ; P)`"
+  also have "... = `($wait \<and> II) \<or> (\<not>$wait \<and> \<delta> ; P)`"
     by (simp add:R3_form)
-  also have "... = `(\<not>ok \<and> $wait \<and> ($tr \<le> $tr\<acute>)) \<or> (ok \<and> $wait \<and> II) \<or> (\<not>$wait \<and> (($tr\<acute> = $tr) \<and> $wait\<acute>) ; II\<^bsub>rea\<^esub>)`"
-    by (simp add:"3")
-  also have "... = `(\<not>ok \<and> $wait \<and> ($tr \<le> $tr\<acute>)) \<or> (ok \<and> $wait \<and> II) \<or> (\<not>$wait \<and> ($tr \<le> $tr\<acute>))`"
-    by (metis "4")
-  also have "... = RH true"
-    by(simp add:RH_def R2_R3_commute R1_R3_commute, simp add:R2_def R1_idempotent R2s_def usubst typing closure defined R1_def R3_form)
-  finally have 5: " \<delta> ; P = RH true " ..
-oops
+  also have "... = `R3(($tr\<acute> = $tr) \<and> $wait\<acute>)`"
+    by (simp add:"3" R3_def CondR_def)
+  finally show ?thesis 
+    by(simp add:\<delta>_def)
+qed
 
 lemma L2 : "P +\<^bsub>ACP\<^esub> P = P" 
-  by(simp add: alternative_def, utp_pred_auto_tac)
+  by(simp add: alternative_def)
 
 lemma L3 : "P +\<^bsub>ACP\<^esub> Q = Q +\<^bsub>ACP\<^esub> P"
   by (metis AndP_comm OrP_comm alternative_def) 
@@ -504,8 +420,336 @@ qed
 lemma L5 : "\<delta> +\<^bsub>ACP\<^esub> Q = Q" 
   by(simp add:alternative_def, utp_pred_auto_tac)
 
+lemma \<delta>_AndP: 
+  assumes "P is ACP1" "P is RH" "P \<in> WF_RELATION"
+  shows "`P \<and> \<delta>` = `P \<and> ($tr\<acute> = $tr) \<and> $wait\<acute>`"
+proof -
+  have "`P \<and> \<delta>` = `R3(P) \<and> \<delta>`" 
+    by (metis assms is_healthy_def RH_is_R3)
+  also have "... = `R3(P \<and> ($tr\<acute> = $tr) \<and> $wait\<acute>)`"
+    by(utp_poly_auto_tac)
+  also have "... = `R3(P) \<and> ($tr\<acute> = $tr) \<and> $wait\<acute>`"
+    apply (utp_poly_auto_tac)
+    apply (simp_all add:closure Rep_binding_ty_def EvalP_SkipR)
+  done
+  finally show ?thesis
+    by (metis AndP_comm Healthy_simp RH_is_R3 assms(2)) 
+qed
+
+lemma NotP_\<delta>_AndP: 
+  assumes "P is ACP1" "P is RH" "P \<in> WF_RELATION"
+  shows "`P \<and> \<not>\<delta>` = `\<not>$wait \<and> P \<and> ($tr\<acute> \<noteq> $tr)`"
+proof -
+have "`P \<and> \<not>\<delta>` = `R3(ACP1(P)) \<and> \<not>\<delta>`" 
+  by(metis assms is_healthy_def RH_is_R3)
+thus ?thesis
+  by (utp_poly_auto_tac)
+qed
+
+lemma ACP1_SemiR_closure: 
+  assumes "P is ACP1" "Q is ACP1" "P \<in> WF_RELATION" "Q \<in> WF_RELATION"
+  shows "P;Q is ACP1"
+
+proof -
+  have "ACP1(P);ACP1(Q) = undefined"
+    apply(simp add:ACP1_def)
+    
+    sorry
+    thus ?thesis sorry
+qed
+
+theorem SemiR_AndP_left_precond_unrest: 
+  assumes
+    "D\<^sub>2 \<sharp> p"
+    "D\<^sub>2 \<sharp> q"
+    "D\<^sub>2 \<sharp> c"
+    "D\<^sub>1 \<sharp> c"
+  shows "(c \<and>\<^sub>p p) ; q = c \<and>\<^sub>p (p ; q)" 
+    apply(subst SemiR_algebraic)
+    apply(simp_all add: assms closure unrest urename)
+    apply(subst RenameP_UNREST [of "D\<^sub>1 \<union> D\<^sub>2"])
+    apply(simp_all add:unrest assms closure)
+    apply(subst SemiR_algebraic)
+    apply(simp_all add: closure assms unrest urename)
+    apply(subst ExistsP_AndP_expand2)
+    apply(simp_all add:assms)
+    apply(subst AndP_assoc[THEN sym])
+    apply(simp)
+done
+
+theorem SemiR_AndP_right_postcond_unrest: 
+  assumes
+    "D\<^sub>2 \<sharp> p"
+    "D\<^sub>2 \<sharp> q"
+    "D\<^sub>2 \<sharp> c"
+    "D\<^sub>0 \<sharp> c"
+  shows "p ; (q \<and>\<^sub>p c) = (p ; q) \<and>\<^sub>p c" 
+    apply(subst SemiR_algebraic)
+    apply(simp_all add: assms closure unrest urename)
+    apply(subst RenameP_UNREST [of "D\<^sub>0 \<union> D\<^sub>2"]) back back
+    apply(simp_all add:unrest assms closure)
+    apply(subst SemiR_algebraic)
+    apply(simp_all add: closure assms unrest urename)
+    apply(subst ExistsP_AndP_expand1)
+    apply(simp_all add:assms)
+    apply(subst AndP_assoc[THEN sym])
+    apply(simp)
+    done
+
+lemma tr_eq_SemiR:
+  assumes "P \<in> WF_RELATION" "Q \<in> WF_RELATION" "P is R1" "Q is R1" 
+  shows "`P;Q \<and> ($tr\<acute> = $tr)` = `(P \<and> ($tr\<acute> = $tr));(Q \<and> ($tr\<acute> = $tr))`"
+proof - 
+  have "`P;Q \<and> ($tr\<acute> = $tr)` = `R1(P);R1(Q) \<and> ($tr\<acute> = $tr)`"
+    by(metis assms is_healthy_def)
+  also have "... = `(\<exists> tr\<acute>\<acute>\<acute> . ($tr \<le> $tr\<acute>\<acute>\<acute>) \<and> (P[$tr\<acute>\<acute>\<acute>/tr\<acute>] ; Q[$tr\<acute>\<acute>\<acute>/tr]) \<and> ($tr\<acute>\<acute>\<acute> \<le> $tr) \<and> ($tr\<acute> = $tr))`"
+  proof -
+    have "`($tr\<acute>\<acute>\<acute> \<le> $tr\<acute>) \<and> ($tr\<acute> = $tr)` = (`($tr\<acute>\<acute>\<acute> \<le> $tr) \<and> ($tr\<acute> = $tr)` :: 'a WF_PREDICATE)"
+     by (utp_poly_auto_tac)
+    thus ?thesis 
+      apply(subst SemiR_extract_variable_ty[of _ _ "tr "])
+      apply(simp_all add:closure unrest assms typing)
+      apply(simp add:R1_def usubst typing defined closure)
+      apply(subst SemiR_AndP_right_postcond_unrest)
+      apply(simp_all add:assms unrest typing defined closure erasure)
+      apply(subst AndP_comm) 
+      apply(subst SemiR_AndP_left_precond_unrest)
+      apply(simp_all add:assms unrest typing defined closure erasure)
+      apply(subst ExistsP_AndP_expand1)
+      apply(simp add:unrest)
+      apply(subst AndP_assoc[THEN sym])  back    
+      apply(subst AndP_assoc[THEN sym])   
+      apply(simp)
+  done
+  qed
+  also have "... = `(\<exists> tr\<acute>\<acute>\<acute>. ($tr = $tr\<acute>\<acute>\<acute>) \<and> ($tr\<acute> = $tr\<acute>\<acute>\<acute>) \<and> P[($tr\<acute>\<acute>\<acute>)/tr\<acute>] ; Q[($tr\<acute>\<acute>\<acute>)/tr])` "
+  proof - 
+    have "`($tr = $tr\<acute>\<acute>\<acute>) \<and> ($tr\<acute> = $tr)` = (`($tr = $tr\<acute>\<acute>\<acute>) \<and> ($tr\<acute> = $tr\<acute>\<acute>\<acute>)` :: 'a WF_PREDICATE)"
+     by (utp_poly_auto_tac)
+   thus ?thesis
+    apply(subst AndP_comm) back
+    apply(subst AndP_assoc[THEN sym])
+    apply(subst AndP_assoc)
+    apply(subst prefix_antisym)
+    apply(simp add:typing closure)
+    apply(subst AndP_assoc)
+    apply(simp add: AndP_assoc[THEN sym])
+    done
+    qed
+  also have "... = `(\<exists> tr\<acute>\<acute>\<acute> . $tr\<acute>\<acute>\<acute> = $tr \<and> P[$tr\<acute>\<acute>\<acute>/tr\<acute>] ; Q[$tr\<acute>\<acute>\<acute>/tr] \<and> $tr\<acute> = $tr\<acute>\<acute>\<acute>)`"
+    by (metis (hide_lams, mono_tags) AndP_comm EqualP_sym calculation)
+  finally show ?thesis
+    apply(simp)
+    apply(rule sym)
+    apply(subst SemiR_extract_variable_ty[of _ _ "tr "])
+    apply(simp_all add:closure assms typing tr_eq_rel_closure)
+    apply(simp add:usubst typing defined closure)
+    apply(subst SemiR_AndP_right_postcond_unrest)
+    apply(simp_all add:assms unrest typing defined closure erasure)
+    apply(subst AndP_comm) 
+    apply(subst SemiR_AndP_left_precond_unrest)
+    apply(simp_all add:assms unrest typing defined closure erasure)
+    apply(subst AndP_assoc[THEN sym])
+    apply(simp)
+   done
+qed
+
+lemma ACP1_tr_eq: 
+  assumes "P \<in> WF_RELATION"
+  shows "`ACP1(P) \<and> ($tr\<acute> = $tr)` =`P \<and> ($tr\<acute> = $tr) \<and> $wait\<acute>`"
+by(utp_poly_auto_tac)
+
+lemma tr_neq_leq:
+  assumes "P \<in> WF_RELATION" "Q \<in> WF_RELATION"
+  shows "`(P \<and> ($tr \<acute> \<noteq> $tr));(Q \<and> ($tr \<le> $tr \<acute>))` = `((P \<and> ($tr \<acute> \<noteq> $tr));(Q \<and> ($tr \<le> $tr \<acute>))) \<and> ($tr \<acute> \<noteq> $tr)`"
+sorry
+
 lemma L6 : 
-  assumes "S is ACP1" "S is RH" "S \<in> WF_RELATION"
-  shows "(P +\<^bsub>ACP\<^esub> Q) ; S = (P;S) +\<^bsub>ACP\<^esub> (Q;S)"
-oops
+  assumes "P is ACP1" "P is RH" "P \<in> WF_RELATION"
+ "Q is ACP1" "Q is RH" "Q \<in> WF_RELATION"
+ "R is ACP1" "R is RH" "R \<in> WF_RELATION"
+  shows "(P +\<^bsub>ACP\<^esub> Q) ; R = (P;R) +\<^bsub>ACP\<^esub> (Q;R)"
+proof -
+  have 1: "`(\<delta> \<and> P \<and> Q) ; R` = `(P \<and> Q \<and> ($tr\<acute> = $tr));($wait \<and> R)`"
+    apply(subst AndP_comm[of "\<delta>"])
+    apply(subst \<delta>_AndP)
+    apply(simp_all add:is_healthy_def ACP1_AndP RH_def R3_AndP R2_AndP R1_AndP)
+    apply(metis assms is_healthy_def)
+    apply(metis assms is_healthy_def RH_is_R3 RH_is_R2 RH_is_R1) 
+    apply(subst AndP_rel_closure)
+    apply(simp_all add:assms)
+    apply(subst SemiR_AndP_right_precond)
+    apply(subst AndP_rel_closure)
+    defer 
+    apply(subst AndP_rel_closure)
+    apply(simp_all add:assms typing closure defined urename AndP_assoc)
+    apply (metis tr_eq_rel_closure)
+
+    done
+    also have "... = `(P \<and> Q \<and> ($tr\<acute> = $tr));($wait \<and> R3(R))`"
+       by(metis assms is_healthy_def RH_is_R3)
+    also have "... = `(P \<and> Q \<and> ($tr\<acute> = $tr));($wait \<and> II)`"
+       apply(simp add:R3_def CondR_def AndP_OrP_distl)
+       by (metis (hide_lams, no_types) AndP_OrP_distl AndP_comm R3_form R3_wait)
+    also have "... = `P \<and> Q \<and> ($tr\<acute> = $tr) \<and> $wait\<acute>`"
+      apply(subst SemiR_AndP_right_precond)
+      apply(subst AndP_rel_closure)
+      defer
+      apply(subst AndP_rel_closure)
+      apply(simp_all add:urename closure typing defined AndP_assoc assms tr_eq_rel_closure)
+      done
+    finally have 1: "`(\<delta> \<and> P \<and> Q) ; R` = `P \<and> Q \<and> ($tr\<acute> = $tr) \<and> $wait\<acute>`"
+      ..
+    have "`\<delta> \<and> (P;R) \<and> (Q;R)` = `(P;R) \<and> (Q;R) \<and> ($tr\<acute> = $tr) \<and> $wait\<acute>`"
+      apply(subst AndP_comm[of "\<delta>"])
+      apply(subst \<delta>_AndP)
+      apply (metis (full_types) ACP1_AndP ACP1_SemiR_closure Healthy_intro Healthy_simp assms(1) assms(3) assms(4) assms(6) assms(7) assms(9))
+      apply (metis RH_AndP_closure RH_SemiR_closure assms(2) assms(3) assms(5) assms(6) assms(8) assms(9))
+      apply (metis AndP_rel_closure SemiR_closure assms(3) assms(6) assms(9))
+      apply(rule AndP_assoc[THEN sym])
+    done
+    also have "... = `((ACP1(P);R3(R)) \<and> ($tr\<acute> = $tr)) \<and> ((ACP1(Q);R3(R)) \<and> ($tr\<acute> = $tr)) \<and> $wait\<acute>`"
+      by (smt AndP_assoc AndP_comm AndP_idem assms is_healthy_def RH_is_R3)
+    also have "... = `((P \<and> ($tr\<acute> = $tr)  \<and> $wait\<acute>) ; (R3(R) \<and> ($tr\<acute> = $tr)) \<and> (Q \<and> ($tr\<acute> = $tr) \<and> $wait\<acute>) ; (R3(R) \<and> ($tr\<acute> = $tr)) \<and> $wait\<acute>)`"
+      apply(subst tr_eq_SemiR)
+      apply(simp_all add:assms closure)
+      apply(metis is_healthy_def assms RH_is_R1 ACP1_R1_commute[THEN sym])
+      apply(metis is_healthy_def assms RH_is_R1 R1_R3_commute)
+      apply(subst ACP1_tr_eq)
+      apply(simp_all add:assms)
+      apply(subst tr_eq_SemiR)
+      apply(simp_all add:assms closure)
+      apply(metis is_healthy_def assms RH_is_R1 ACP1_R1_commute[THEN sym])
+      apply(metis is_healthy_def assms RH_is_R1 R1_R3_commute)
+      apply(subst ACP1_tr_eq)
+      apply(simp_all add:assms)
+      done
+    also have "... = `((P \<and> ($tr\<acute> = $tr)) ; ($wait \<and> R3(R) \<and> ($tr\<acute> = $tr)) \<and> (Q \<and> ($tr\<acute> = $tr)) ; ($wait \<and> R3(R) \<and> ($tr\<acute> = $tr)) \<and> $wait\<acute>)`"
+      apply(subst SemiR_AndP_right_precond) back back
+      apply(simp_all add:typing closure defined assms tr_eq_rel_closure urename)
+      apply(subst SemiR_AndP_right_precond) back back back
+      apply(simp_all add:typing closure defined assms tr_eq_rel_closure urename AndP_assoc)
+      done
+    also have "... = `P \<and> Q \<and> ($tr\<acute> = $tr) \<and> $wait\<acute>`"
+      apply(simp add: AndP_assoc AndP_comm[of "`$wait`"] R3_wait)
+      apply(simp add: AndP_comm[of "`$wait`",THEN sym] AndP_assoc[THEN sym])
+      apply(subst SemiR_AndP_right_precond)
+      apply(simp_all add:typing closure defined assms urename tr_eq_rel_closure)
+      apply(subst SemiR_AndP_right_precond) back
+      apply(simp_all add:typing closure defined assms urename tr_eq_rel_closure SkipR_as_SkipRA)
+      apply(subst SkipRA_unfold[of "tr \<down>"])
+      apply(simp_all add:closure)
+      apply(subst SkipRA_unfold[of "tr \<down>"]) back
+      apply(simp_all add:closure)
+      apply(simp add:erasure typing defined closure AndP_assoc[THEN sym])
+      apply(subst AndP_comm) back back back
+      apply(subst AndP_comm) back back back back back back back back
+      apply(simp add:AndP_assoc)
+      apply(subst SkipRA_unfold[of "tr \<down>",THEN sym])
+      apply(simp_all add:closure)
+      apply(subst SkipRA_unfold[of "tr \<down>",THEN sym])
+      apply(simp_all add:closure SkipR_as_SkipRA[THEN sym])
+      apply(utp_poly_auto_tac)
+      done
+    finally have 2: "`(\<delta> \<and> P \<and> Q) ; R` = `\<delta> \<and> (P;R) \<and> (Q;R)`"
+      by(simp add:1)
+  have A: "`(\<not>\<delta> \<and> P);R` = `\<not>$wait \<and> (P \<and> ($tr\<acute> \<noteq> $tr));R`"
+    apply(subst AndP_comm[of "`\<not>\<delta>`"])
+    apply(subst NotP_\<delta>_AndP)
+    apply(simp_all add:assms)
+    apply(subst SemiR_AndP_left_precond)
+    apply(simp_all add:assms closure tr_eq_rel_closure)
+    done
+  have B: "`\<not>\<delta> \<and> (P;R)` =`\<not>$wait \<and> (P;R) \<and> ($tr\<acute> \<noteq> $tr)`"
+    apply(subst AndP_comm[of "`\<not>\<delta>`"])
+    apply(subst NotP_\<delta>_AndP)
+    apply(subst ACP1_SemiR_closure)
+    apply(simp_all add:assms closure)
+    apply(subst RH_SemiR_closure)
+    apply(simp_all add:assms)
+    done
+  also have "... = `\<not>$wait \<and> ((P \<and> (($tr\<acute> = $tr) \<or> ($tr\<acute> \<noteq> $tr)));R) \<and> ($tr\<acute> \<noteq> $tr)`"
+    by (smt AndP_OrP_distl AndP_comm WF_PREDICATE_cases)
+  also have "... = `\<not>$wait \<and> (((ACP1(P) \<and> ($tr\<acute> = $tr)) ; R3(R)) \<or> ((P \<and> ($tr\<acute> \<noteq> $tr)) ; R)) \<and>  ($tr\<acute> \<noteq> $tr)`"
+    apply(simp add:AndP_OrP_distl SemiR_OrP_distr)
+    apply(metis assms is_healthy_def RH_is_R3)
+    done
+  also have "... = `\<not>$wait \<and> ((P \<and> ($tr\<acute> = $tr)) ; ($wait \<and> R3(R)) \<or> ((P \<and> ($tr\<acute> \<noteq> $tr)) ; R)) \<and> ($tr\<acute> \<noteq> $tr)`" 
+    apply(subst ACP1_tr_eq)
+    apply(simp add:assms)
+    apply(subst SemiR_AndP_right_precond)
+    apply(simp_all add:closure typing defined assms tr_eq_rel_closure AndP_assoc[THEN sym] urename)
+    done
+  also have "... = `\<not>$wait \<and> ((P \<and> ($tr\<acute> \<noteq> $tr)) ; R1(R)) \<and> ($tr\<acute> \<noteq> $tr)`"
+    apply(simp add: AndP_comm[of "`$wait`"] R3_wait)
+    apply(simp add: AndP_comm[of _ "`$wait`"])
+    apply(subst SemiR_AndP_right_precond)
+    apply(simp_all add:typing defined closure assms urename tr_eq_rel_closure AndP_assoc[THEN sym] AndP_OrP_distr)
+    apply(subst AndP_comm) back back back
+    apply(subst AndP_comm) back
+    apply(simp add:AndP_assoc)
+    apply(subst AndP_contra[of "`($tr\<acute> = $tr)`"])
+    apply(simp add:AndP_assoc[THEN sym])
+    apply(metis assms is_healthy_def RH_is_R1)
+    done
+  also have "... = `\<not>$wait \<and> ((P \<and> ($tr\<acute> \<noteq> $tr)) ; R1(R))`"
+    apply(simp add:R1_def)
+    apply(subst tr_neq_leq) back
+    apply(simp_all add:assms)
+    done
+  finally have 3: "`(\<not>\<delta> \<and> P);R` = `\<not>\<delta> \<and> (P;R)`" 
+    apply(simp add:A)
+    apply(metis assms is_healthy_def RH_is_R1)
+    done
+  have A: "`(\<not>\<delta> \<and> Q);R` = `\<not>$wait \<and> (Q \<and> ($tr\<acute> \<noteq> $tr));R`"
+    apply(subst AndP_comm[of "`\<not>\<delta>`"])
+    apply(subst NotP_\<delta>_AndP)
+    apply(simp_all add:assms)
+    apply(subst SemiR_AndP_left_precond)
+    apply(simp_all add:assms closure tr_eq_rel_closure)
+    done
+  have B: "`\<not>\<delta> \<and> (Q;R)` =`\<not>$wait \<and> (Q;R) \<and> ($tr\<acute> \<noteq> $tr)`"
+    apply(subst AndP_comm[of "`\<not>\<delta>`"])
+    apply(subst NotP_\<delta>_AndP)
+    apply(subst ACP1_SemiR_closure)
+    apply(simp_all add:assms closure)
+    apply(subst RH_SemiR_closure)
+    apply(simp_all add:assms)
+    done
+  also have "... = `\<not>$wait \<and> ((Q \<and> (($tr\<acute> = $tr) \<or> ($tr\<acute> \<noteq> $tr)));R) \<and> ($tr\<acute> \<noteq> $tr)`"
+    by (smt AndP_OrP_distl AndP_comm WF_PREDICATE_cases)
+  also have "... = `\<not>$wait \<and> (((ACP1(Q) \<and> ($tr\<acute> = $tr)) ; R3(R)) \<or> ((Q \<and> ($tr\<acute> \<noteq> $tr)) ; R)) \<and>  ($tr\<acute> \<noteq> $tr)`"
+    apply(simp add:AndP_OrP_distl SemiR_OrP_distr)
+    apply(metis assms is_healthy_def RH_is_R3)
+    done
+  also have "... = `\<not>$wait \<and> ((Q \<and> ($tr\<acute> = $tr)) ; ($wait \<and> R3(R)) \<or> ((Q \<and> ($tr\<acute> \<noteq> $tr)) ; R)) \<and> ($tr\<acute> \<noteq> $tr)`" 
+    apply(subst ACP1_tr_eq)
+    apply(simp add:assms)
+    apply(subst SemiR_AndP_right_precond)
+    apply(simp_all add:closure typing defined assms tr_eq_rel_closure AndP_assoc[THEN sym] urename)
+    done
+  also have "... = `\<not>$wait \<and> ((Q \<and> ($tr\<acute> \<noteq> $tr)) ; R1(R)) \<and> ($tr\<acute> \<noteq> $tr)`"
+    apply(simp add: AndP_comm[of "`$wait`"] R3_wait)
+    apply(simp add: AndP_comm[of _ "`$wait`"])
+    apply(subst SemiR_AndP_right_precond)
+    apply(simp_all add:typing defined closure assms urename tr_eq_rel_closure AndP_assoc[THEN sym] AndP_OrP_distr)
+    apply(subst AndP_comm) back back back
+    apply(subst AndP_comm) back
+    apply(simp add:AndP_assoc)
+    apply(subst AndP_contra[of "`($tr\<acute> = $tr)`"])
+    apply(simp add:AndP_assoc[THEN sym])
+    apply(metis assms is_healthy_def RH_is_R1)
+    done
+  also have "... = `\<not>$wait \<and> ((Q \<and> ($tr\<acute> \<noteq> $tr)) ; R1(R))`"
+    apply(simp add:R1_def)
+    apply(subst tr_neq_leq) back
+    apply(simp_all add:assms)
+    done
+  finally have 4: "`(\<not>\<delta> \<and> Q);R` = `\<not>\<delta> \<and> (Q;R)`" 
+    apply(simp add:A)
+    apply(metis assms is_healthy_def RH_is_R1)
+    done
+  show ?thesis
+    by(simp add:alternative_def CondR_def SemiR_OrP_distr AndP_OrP_distl 2 3 4)
+qed
 end
