theories/theories/utp_reactive.thy
@@ -8,7 +8,6 @@ header {* Reactive Processes *}
 
 theory utp_reactive
 imports 
-  utp_designs
   utp_theory
   "reactive/utp_reactive_lemmas"
 begin
@@ -17,18 +16,7 @@ default_sort REACTIVE_SORT
 
 abbreviation "ref  \<equiv> MkPlainP ''ref'' True TYPE('m EVENT USET) TYPE('m)"
 
-abbreviation "REA \<equiv> OKAY \<union> {wait\<down>, wait\<down>\<acute>, tr\<down>, tr\<down>\<acute>, ref\<down>, ref\<down>\<acute>}"
-
-definition SkipREA :: "'a WF_PREDICATE" where
-"SkipREA = `(\<not> ok \<and> ($tr \<le> $tr\<acute>)) \<or> (ok' \<and> II\<^bsub>REL_VAR - OKAY\<^esub>)`"
-
-syntax 
-  "_upred_skiprea" :: " upred" ("II\<^bsub>rea\<^esub>")
-
-translations
-  "_upred_skiprea" == "CONST SkipREA"
-
-declare SkipREA_def [eval, evalr, evalp]
+abbreviation "REA \<equiv> {wait\<down>, wait\<down>\<acute>, tr\<down>, tr\<down>\<acute>, ref\<down>, ref\<down>\<acute>}"
 
 text {* R1 ensures that the trace only gets longer *}
 
@@ -44,7 +32,7 @@ definition R2 :: "'a WF_PREDICATE \<Rightarrow> 'a WF_PREDICATE" where
 "R2(P) = R1 (R2s P)"
 
 definition R3 :: "'a WF_PREDICATE \<Rightarrow> 'a WF_PREDICATE" where
-"R3(P) = `II\<^bsub>rea\<^esub> \<lhd> $wait \<rhd> P`"
+"R3(P) = `II \<lhd> $wait \<rhd> P`"
 
 definition RH :: "'a WF_PREDICATE \<Rightarrow> 'a WF_PREDICATE" where 
 "RH P = (R1 \<circ> R2 \<circ> R3)P"
@@ -54,7 +42,6 @@ declare R2_def [eval, evalr, evalrr, evalrx, evalp]
 declare R2s_def [eval, evalr, evalrr, evalrx, evalp]
 declare R3_def [eval, evalr, evalrr, evalrx, evalp]
 declare is_healthy_def [eval, evalr, evalrr, evalrx, evalp]
-declare SkipREA_def [eval, evalr, evalrr, evalrx, evalp]
 declare RH_def [eval, evalr, evalrr, evalrx, evalp]
 
 subsection {* Closure Laws *}
@@ -62,10 +49,6 @@ subsection {* Closure Laws *}
 lemma WF_RELATION_UNREST:
   "NON_REL_VAR \<sharp> P \<Longrightarrow> P \<in> WF_RELATION"
   by (simp add:WF_RELATION_def)
-
-lemma SkipREA_rel_closure [closure]:
-  "`II\<^bsub>rea\<^esub>` \<in> WF_RELATION"
-  by (simp add:SkipREA_def closure unrest erasure WF_RELATION_UNREST)
 
 lemma R1_rel_closure [closure]:
   "P \<in> WF_RELATION \<Longrightarrow> R1(P) \<in> WF_RELATION"
@@ -99,231 +82,12 @@ lemma Aida : "`(($tr \<le> $tr\<acute>) ; ((\<not>ok \<and> $wait) \<and> ($tr \
   apply (metis tr_leq_trans)
 done
     
-lemma Aidb : "`$okay \<and> ($okay\<acute> = $okay)` = `$okay \<and> $okay\<acute>`" by (utp_poly_auto_tac)
-lemma Aidc : "`$wait \<and> ($wait\<acute> = $wait)` = `$wait \<and> $wait\<acute>`" by (utp_poly_auto_tac)
-lemma Aidd : "`II\<^bsub>REL_VAR - OKAY\<^esub>\<^sub>t`=`$wait\<acute> \<and> II\<^bsub>REL_VAR - OKAY - {wait\<down>, wait\<down>\<acute>}\<^esub>`"
-  apply (subst SkipRA_unfold[of "wait \<down>"])
-  apply (simp_all)
-  apply (metis MkPlain_UNDASHED PVAR_VAR_MkPVAR)
-  apply (metis MkPlain_UNDASHED PVAR_VAR_MkPVAR UNDASHED_dash_DASHED)
-  apply (metis MkPlainP_UNDASHED PVAR_VAR_PUNDASHED_UNDASHED) 
-  apply (utp_pred_auto_tac)
-  apply (simp add: usubst typing closure defined)
-  apply (subst VarP_EqualP_aux)
-  apply (simp_all add:typing erasure)
-done
+lemma Aidc : "`$wait \<and> ($wait\<acute> = $wait)` = `$wait \<and> $wait\<acute>`" by utp_poly_auto_tac
 
-subsection {* SkipREA Laws *}
-
-(* Additional lemmas *)
-
-declare EvalP_SkipRA [evalp]
-
-thm EvalP_SkipRA
-
-lemma TypeUSound_ProjU_inj [simp]:
-  fixes x :: "'m :: VALUE"
-  assumes "(ProjU x :: 'a) = (ProjU y :: 'a)" "TYPEUSOUND('a :: DEFINED, 'm :: VALUE)" 
-          "x :! TYPEU('a)" "y :! TYPEU('a)"
-  shows "x = y"
-    by (metis TypeUSound_ProjU_inv assms)
-
-lemma binding_ty_transfer [evalp]:
-  fixes x :: "('a :: DEFINED, 'm :: VALUE) PVAR"
-  assumes "TYPEUSOUND('a, 'm)" "pvaux x" "pvaux y"
-  shows "\<langle>b1\<rangle>\<^sub>b x\<down> = \<langle>b2\<rangle>\<^sub>b y\<down> \<longleftrightarrow> \<langle>b1\<rangle>\<^sub>* x = \<langle>b2\<rangle>\<^sub>* y"
-  apply (auto simp add:Rep_binding_ty_def typing assms)
-  apply (drule TypeUSound_ProjU_inj)
-  apply (simp_all add:assms typing defined)
-  apply (rule typing)
-  apply (simp_all)
-  apply (metis assms(2) pvaux_aux)
-  apply (rule typing)
-  apply (simp_all)
-  apply (metis assms(3) pvaux_aux)
-done
-
-lemma binding_ty_transfer_dl [evalp]:
-  fixes x :: "('a :: DEFINED, 'm :: VALUE) PVAR"
-  assumes "TYPEUSOUND('a, 'm)" "pvaux x" "pvaux y"
-  shows "\<langle>b1\<rangle>\<^sub>b x\<down> = \<langle>b2\<rangle>\<^sub>b y\<down>\<acute> \<longleftrightarrow> \<langle>b1\<rangle>\<^sub>* x = \<langle>b2\<rangle>\<^sub>* y\<acute>"
-  apply (subst binding_ty_transfer[THEN sym])
-  apply (simp_all add:assms)
-done
-
-lemma SkipRA_is_R1 : 
-  "`R1(II\<^bsub>REL_VAR - OKAY\<^esub>)` = `II\<^bsub>REL_VAR - OKAY\<^esub>`"
-  apply (auto simp add:evalp var_dist closure)
-  apply (drule_tac x="tr\<down>" in bspec)
-  apply (simp_all add:closure evalp typing defined)
-done
-
-lemma tr_conserved_is_R1 : "`R1($tr\<acute> = $tr)` = `($tr\<acute> = $tr)`" 
-  by (simp add:R1_def, utp_poly_auto_tac)
+lemma tr_conserved_is_R1 : "`R1($tr\<acute> = $tr)` = `($tr\<acute> = $tr)`" by(simp add:R1_def, utp_poly_auto_tac)
 
 lemma R1_monotonic: "P \<sqsubseteq> Q \<Longrightarrow> R1(P) \<sqsubseteq> R1(Q)" 
   by utp_pred_tac
-
-(*L1 H1-wait-okay' *)
-
-lemma H1_wait_true: 
-  "(H1(P))\<^sub>t = H1(P\<^sub>t)"
-by(utp_pred_auto_tac)
-
-lemma H1_wait_false: 
-  "(H1(P))\<^sub>f = H1(P\<^sub>f)"
-by(utp_pred_auto_tac)
-
-lemma H1_okay'_true: 
-  "(H1(P))\<^sup>t = H1(P\<^sup>t)"
-by(utp_pred_auto_tac)
-
-lemma H1_okay'_false: 
-  "(H1(P))\<^sup>f = H1(P\<^sup>f)"
-by(utp_pred_auto_tac)
-
-(*L3 II_rea-II_rel-conditional *)
-
-lemma SkipREA_CondR_SkipR: 
-  "`II\<^bsub>rea\<^esub>` = `II \<lhd> ok \<rhd> ($tr \<le> $tr\<acute>)`"
-proof -
-  have "`II \<lhd> ok \<rhd> ($tr \<le> $tr\<acute>)` = `($okay\<acute> = $okay \<and> II\<^bsub>REL_VAR - OKAY\<^esub>) \<lhd> ok \<rhd> ($tr \<le> $tr\<acute>)`"
-    by (simp add:SkipR_as_SkipRA SkipRA_unfold[of "okay\<down>"] closure erasure typing)
-
-  also 
-  have "... = `($okay\<acute> = $okay \<and> II\<^bsub>REL_VAR - OKAY\<^esub>)[true/okay] 
-               \<lhd> ok \<rhd> 
-               (($tr \<le> $tr\<acute>)[false/okay])`"
-    by (simp add:erasure, rule_tac CondR_VarP_aux[of "okay\<down>"], simp_all)
-
-  also have "... = `(ok' \<and> II\<^bsub>REL_VAR - OKAY\<^esub>) \<lhd> ok \<rhd> ($tr \<le> $tr\<acute>)`"
-    by (simp add:usubst typing defined closure)
-
-  also have "... = `(ok \<and> ok' \<and> II\<^bsub>REL_VAR - OKAY\<^esub>) \<or> (\<not> ok \<and> ($tr \<le> $tr\<acute>))`"
-    by (utp_pred_auto_tac)
-
-  also have "... = `II\<^bsub>rea\<^esub>`"
-    apply (simp add:SkipREA_def)
-    apply (rule_tac x="okay\<down>" in BoolType_aux_var_split_eq_intro)
-    apply (simp_all add:usubst closure typing defined urename)
-    apply (utp_poly_auto_tac)
-    apply (drule_tac x="tr\<down>" in bspec)
-    apply (simp_all add:var_dist closure evalp typing)
-  done
-  finally show ?thesis ..
-qed
-
-(*L2 II_rea-II_rel *)
-
-lemma SkipREA_SkipR: 
-  "`II\<^bsub>rea\<^esub>` = `(\<not> ok \<and> ($tr \<le> $tr\<acute>)) \<or> II`"
-proof -
-  have "`II\<^bsub>rea\<^esub>` = `(\<not> ok \<and> ($tr \<le> $tr\<acute>)) \<or> (ok \<and> II)`" by(simp add: OrP_comm SkipREA_CondR_SkipR CondR_def)
-  also have "... = `(\<not> ok \<and> ($tr \<le> $tr\<acute>)) \<or> (\<not> ok \<and> ($tr \<le> $tr\<acute>) \<and> II) \<or> (ok \<and> II)`" by utp_pred_auto_tac
-  also have "... = `(\<not> ok \<and> ($tr \<le> $tr\<acute>)) \<or> (\<not> ok \<and> II) \<or> (ok \<and> II)`"
-  proof -
-    have "`($tr \<le> $tr\<acute>) \<and> II` = `R1(II)`"
-      by utp_pred_auto_tac
-    also have "... = `R1($tr\<acute> = $tr) \<and> II\<^bsub>REL_VAR - {tr\<down>,tr\<down>\<acute>}\<^esub>`"
-      apply(simp add:SkipR_as_SkipRA)
-      apply(subst SkipRA_unfold[of "tr \<down>"])
-      apply(simp_all)
-      apply(metis MkPlain_UNDASHED PVAR_VAR_MkPVAR)
-      apply(metis MkPlain_UNDASHED PVAR_VAR_MkPVAR UNDASHED_dash_DASHED)
-      apply(metis MkPlain_UNDASHED PVAR_VAR_MkPVAR)
-      apply(simp add:typing closure defined erasure)
-      apply(utp_pred_auto_tac)
-      done
-    also have "... = `($tr\<acute> = $tr) \<and> II\<^bsub>REL_VAR - {tr\<down>,tr\<down>\<acute>}\<^esub>`"
-      by(utp_poly_auto_tac)
-    finally have "`($tr \<le> $tr\<acute>) \<and> II` = `II`" 
-      apply(simp add: SkipR_as_SkipRA)
-      apply(subst SkipRA_unfold[of "tr \<down>"]) back
-      apply(simp_all)
-      apply(metis MkPlain_UNDASHED PVAR_VAR_MkPVAR)
-      apply(metis MkPlain_UNDASHED PVAR_VAR_MkPVAR UNDASHED_dash_DASHED)
-      apply(metis MkPlain_UNDASHED PVAR_VAR_MkPVAR)
-      apply(simp add:typing closure defined erasure)
-      done 
-    thus ?thesis by metis
-  qed
-  finally show ?thesis by utp_pred_auto_tac
-qed
-
-(*L4 okay-II_rea-II_rel *)
-
-lemma ok_SkipREA_SkipR : 
-  "`ok \<and> II\<^bsub>rea\<^esub>` = `ok \<and> II`"
-proof -
-  have "`ok \<and> II\<^bsub>rea\<^esub>` = `ok \<and> ok' \<and> II\<^bsub>REL_VAR - OKAY\<^esub>`" 
-    by(utp_pred_auto_tac)
-  also have "... = `ok \<and> II\<^bsub>REL_VAR\<^esub>`" 
-  proof -
-      have "`ok \<and> ok'` = `ok \<and> ($okay\<acute> = $okay)`"
-        by (metis Aidb)
-      thus ?thesis
-        apply(simp add: SkipRA_unfold[of "okay \<down>"] closure erasure typing defined)
-        apply(utp_pred_auto_tac)
-        done
-  qed
-  finally show ?thesis 
-    by (metis SkipR_as_SkipRA)
-qed
-
-(*L5 okay-II_rea-sequence-unit *)
-
-lemma okay_SkipREA_sequence_unit : 
-assumes 
-  "P \<in> WF_RELATION"
-shows
-  "`(ok \<and> II\<^bsub>rea\<^esub>) ; P` = `ok \<and> P`"
-proof -
-  have "`(ok \<and> II\<^bsub>rea\<^esub>) ; P` = `(ok \<and> II) ; P`" 
-    by (metis ok_SkipREA_SkipR)
-  also  have "... = `ok \<and> (II ; P)`"
-    by (subst SemiR_AndP_left_precond, simp_all add:SkipR_closure assms MkPlainP_UNDASHED PUNDASHED_WF_CONDITION)
-  finally show ?thesis 
-    by(simp)
-qed
-
-(*L6 II_rea-H2 *)
-
-lemma H2_SkipREA:
-  "`H2(II\<^bsub>rea\<^esub>)` = `II\<^bsub>rea\<^esub>`"
-proof -
-  have "`H2(II\<^bsub>rea\<^esub>)` = `II\<^bsub>rea\<^esub>\<^sup>f \<or> (II\<^bsub>rea\<^esub>\<^sup>t \<and> ok')`"
-    by (simp add:H2_def J_split closure)
-
-  also have "... = `(\<not> ok \<and> ($tr \<le> $tr\<acute>)) \<or> II\<^bsub>REL_VAR - OKAY\<^esub> \<and> ok'`"
-    apply (simp add:SkipREA_def usubst typing defined closure)
-    apply (utp_pred_auto_tac)
-  done
-
-  also have "... = `II\<^bsub>rea\<^esub>`"
-    apply (simp add:SkipREA_def)
-    apply (utp_pred_auto_tac)
-  done
-
-  finally show ?thesis .
-qed
-
-(*L7 H1-II_rea-II_rel *)
-
-lemma H1_SkipREA: 
-  "`H1(II\<^bsub>rea\<^esub>)` = `H1(II)`"
-proof -
-  have "`H1(II\<^bsub>rea\<^esub>)` = `ok \<Rightarrow> II\<^bsub>rea\<^esub>`"
-    by (simp add:H1_def)
-
-  also have "... = `ok \<Rightarrow> (II \<lhd> ok \<rhd> ($tr \<le> $tr\<acute>))`"
-    by (simp add:SkipREA_CondR_SkipR)
-
-  also have "... = `ok \<Rightarrow> II`"
-    by (metis (lifting, no_types) CondR_true_cond ImpliesP_export)
-
-  finally show ?thesis
-    by (simp add:H1_def)
-qed
 
 subsection {* R1 Laws *}
 
@@ -363,23 +127,15 @@ lemma R1_negate_R1:
   "`R1(\<not>R1(P))` = `R1(\<not>P)`"
   by(utp_pred_auto_tac)
   
-(* L7 R1-wait-okay' *)
+(* L7 R1-wait *)
 
 lemma R1_wait_true: 
   "(R1(P))\<^sub>t = R1(P\<^sub>t)"
-by(utp_poly_auto_tac)
+by(simp add:R1_def, utp_poly_auto_tac)
 
 lemma R1_wait_false: 
   "(R1(P))\<^sub>f = R1(P\<^sub>f)"
-by(utp_poly_auto_tac)
-
-lemma R1_okay'_true: 
-  "(R1(P))\<^sup>t = R1(P\<^sup>t)"
-by(utp_poly_auto_tac)
-
-lemma R1_okay'_false: 
-  "(R1(P))\<^sup>f = R1(P\<^sup>f)"
-by(utp_poly_auto_tac)
+by(simp add:R1_def, utp_poly_auto_tac)
 
 (* L8 II_rel-R1 *)
 
@@ -389,17 +145,9 @@ lemma R1_SkipR:
 
 (* L9 II_rea-R1 *)
 
-lemma R1_SkipREA:
-  "`R1(II\<^bsub>rea\<^esub>)` = `II\<^bsub>rea\<^esub>`"
-  by (auto simp add:eval evalp closure Rep_binding_ty_def)
-
 lemma R1_tr_leq_tr':
   "`R1($tr \<le> $tr\<acute>)` = `$tr \<le> $tr\<acute>`"
   by (simp add:R1_def)
-
-lemma SkipREA_is_R1:
-  "`R1(II\<^bsub>rea\<^esub>)` = `II\<^bsub>rea\<^esub>`"
-  by (simp add:SkipREA_CondR_SkipR R1_CondR R1_SkipR R1_tr_leq_tr')
 
 (* L10 R1-\<and>-closure *)
 
@@ -441,38 +189,15 @@ theorem R1_SemiR_closure [closure]:
   apply (simp add:tr_leq_trans)
 done
 
-(* L14 II_rea-R1-H1 *)
-
-lemma SkipREA_R1_H1: 
-  "`II\<^bsub>rea\<^esub>` = `R1(H1(II\<^bsub>rea\<^esub>))`"
-proof -
-  from SkipREA_is_R1 have "`II\<^bsub>rea\<^esub>` = `R1(II\<^bsub>rea\<^esub>)`" 
-    ..
-  thus ?thesis 
-    by(utp_pred_auto_tac)
-qed
-
-(* L15 R1-H2-commutativity *)
-
-lemma R1_H2_commute:
-  assumes "P \<in> WF_RELATION"
-  shows "H2(R1(P)) = R1(H2(P))"
-  apply (simp add: H2_def J_split unrest closure)
-  apply (subst J_split)
-  apply (metis R1_rel_closure assms)
-  apply (subst J_split)
-  apply (metis assms)
-  apply (simp add: R1_def usubst typing defined)
-  apply (utp_pred_auto_tac)
-done
-
 subsection {* R2 Laws *}
 
 (* L3 R2-idempotent *)
 
 lemma R2s_idempotent: "`R2s(R2s(P))` = `R2s(P)`"
   apply (simp add:R2s_def)
-  apply (subst SubstP_twice_3) back
+  apply (subst SubstP_twice_2) back
+  apply (simp_all add:typing defined closure unrest)
+  apply (subst SubstP_twice_1) 
   apply (simp_all add:typing defined closure unrest)
   apply (simp add:usubst typing defined closure)
 done
@@ -532,10 +257,10 @@ by(utp_pred_auto_tac)
 lemma R2_CondR_closure_2: 
 assumes "P is R2" "Q is R2" "b is R2"
 shows "`P \<lhd> b \<rhd> Q` is R2"
-using assms
+using assms 
 proof -
   have "`R2(P \<lhd> b \<rhd> Q)`  = `(R2(b) \<and> R2(P)) \<or> (R1(\<not> R2(b)) \<and> R2(Q))`"
-    by(simp add:CondR_def R2_OrP R2_AndP R2_negate)
+    by (utp_poly_auto_tac)
   also have "... = `(R2(b) \<and> R2(P)) \<or> (\<not> R2(b) \<and> R2(Q))`"
     by(utp_pred_auto_tac)
   also from assms have "... = `(b \<and> P) \<or> (\<not> b \<and> Q)`" 
@@ -556,64 +281,439 @@ assumes "P is R2" "Q is R2"
 shows "`P \<lhd> ($tr\<acute> = $tr) \<rhd> Q` is R2"
 by(subst R2_CondR_closure_2, simp_all add:assms, simp add:is_healthy_def tr_conserved_is_R2)
 
+lemma RenamePV_aux [simp]:
+  "pvaux (ss\<bullet>x) = pvaux x"
+  by (metis PVAR_VAR_RENAME Rep_VAR_RENAME_aux pvaux_aux)
+
+lemma SS1_UNREST_d3 [unrest]:
+  "P \<in> WF_RELATION \<Longrightarrow> {x\<acute>\<acute>\<acute>} \<sharp> (SS1\<bullet>P)"
+  apply (rule UNREST_RenameP[of "{x\<acute>\<acute>\<acute>}"])
+  apply (simp_all add:unrest urename)
+done
+
+lemma SS2_UNREST_d3 [unrest]:
+  "P \<in> WF_RELATION \<Longrightarrow> {x\<acute>\<acute>\<acute>} \<sharp> (SS2\<bullet>P)"
+  apply (rule UNREST_RenameP[of "{x\<acute>\<acute>\<acute>}"])
+  apply (simp_all add:unrest urename)
+done
+
 (* L9 R2-composition *)
 (*R2 *)
 
+
+abbreviation "tt1   \<equiv> MkPlainP ''tt1'' True TYPE('m EVENT ULIST) TYPE('m)"
+abbreviation "tt2   \<equiv> MkPlainP ''tt2'' True TYPE('m EVENT ULIST) TYPE('m)"
+abbreviation "tt   \<equiv> MkPlainP ''tt'' True TYPE('m EVENT ULIST) TYPE('m)"
+
+lemma R2_form:
+  assumes "P \<in> WF_RELATION" "pvaux ttx" 
+  shows "R2(P) = (\<exists>\<^sub>p {ttx\<down>\<acute>\<acute>\<acute>} . `P[\<langle>\<rangle>/tr][$ttx\<acute>\<acute>\<acute>/tr\<acute>] \<and> ($tr\<acute> = $tr ^ $ttx\<acute>\<acute>\<acute>)`)"
+proof -
+have "`$tr \<le> $tr\<acute>` = (\<exists>\<^sub>p {ttx\<down>\<acute>\<acute>\<acute>} . `$tr\<acute> = $tr ^ $ttx\<acute>\<acute>\<acute>`)"
+  by (metis (hide_lams, no_types) PVAR_VAR_pvdash assms(2) tr_prefix_as_concat)
+hence "R2(P) = R2s(P) \<and>\<^sub>p (\<exists>\<^sub>p {ttx\<down>\<acute>\<acute>\<acute>} .  `$tr\<acute> = $tr ^ $ttx\<acute>\<acute>\<acute>`)"
+  by(metis R2_def R1_def)
+also have "... = (\<exists>\<^sub>p {ttx\<down>\<acute>\<acute>\<acute>} . R2s(P) \<and>\<^sub>p `$tr\<acute> = $tr ^ $ttx\<acute>\<acute>\<acute>`)"
+  apply(subst ExistsP_AndP_expand2)
+  apply(rule unrest)
+  apply(simp_all add:unrest assms closure)
+  done  
+also have "... = (\<exists>\<^sub>p {ttx\<down>\<acute>\<acute>\<acute>} . `$tr\<acute> = $tr ^ $ttx\<acute>\<acute>\<acute>  \<and> R2s(P)`)"
+  by(subst AndP_comm, simp)
+also have  "... = (\<exists>\<^sub>p {ttx\<down>\<acute>\<acute>\<acute>} . `R2s(P)[($tr ^ $ttx\<acute>\<acute>\<acute>)/tr\<acute>] \<and> $tr\<acute> = $tr ^ $ttx\<acute>\<acute>\<acute>`)"
+  apply(simp add:erasure typing defined closure)
+  apply(subst EqualP_SubstP)
+  apply(simp_all add: typing defined closure assms AndP_comm)
+  done
+also have "... = (\<exists>\<^sub>p {ttx\<down>\<acute>\<acute>\<acute>} . `P[\<langle>\<rangle>/tr][$ttx\<acute>\<acute>\<acute>/tr\<acute>] \<and> ($tr\<acute> = $tr ^ $ttx\<acute>\<acute>\<acute>)`)" 
+  apply(simp add:R2s_def)
+  apply(subst SubstP_twice_1)
+  apply(simp_all add:typing defined closure assms)
+  apply(simp add:usubst typing defined closure assms)
+  apply(subst app_minus)
+  apply(simp_all add:typing closure)
+  done 
+finally show ?thesis 
+  by (metis assms(1))
+qed  
+
+lemma SS_rel_closure [closure]:
+  "P \<in> WF_RELATION \<Longrightarrow> SS\<bullet>P \<in> WF_RELATION"
+  by (metis ConvR_def ConvR_rel_closure)
+
+lemma append_assoc:
+  fixes xs ys zs :: "(('a :: DEFINED) ULIST, 'm :: LIST_SORT) PVAR"
+  shows "|($xs ^ $ys) ^ $zs| = |$xs ^ ($ys ^ $zs)|"
+  by (utp_poly_tac)
+
 (*
+lemma "x \<in> PUNDASHED \<Longrightarrow> SS2 \<bullet> x\<acute>\<acute>\<acute> = x\<acute>\<acute>\<acute>"
+*)
+
+lemma EvalP_ExistsP_singleton_d3_pvaux_ty [evalp]:
+  fixes x :: "('a :: DEFINED, 'm :: VALUE) PVAR"
+  assumes "TYPEUSOUND('a, 'm)" "pvaux x"
+  shows "\<lbrakk>\<exists>\<^sub>p {x\<down>\<acute>\<acute>\<acute>} . p\<rbrakk>b = (\<exists> v . v \<rhd>\<^sub>p x\<acute>\<acute>\<acute> \<and> \<lbrakk>p\<rbrakk>(b(x\<acute>\<acute>\<acute> :=\<^sub>* v)))"
+  apply (subst EvalP_ExistsP_singleton_pvaux_ty[THEN sym])
+  apply (simp_all add:assms)
+done
+
+lemma R2_SemiR_form: 
+  assumes "P \<in> WF_RELATION" "Q \<in> WF_RELATION"
+  shows "R2(P);R2(Q) =  `(\<exists> tt1\<acute>\<acute>\<acute>. \<exists> tt2\<acute>\<acute>\<acute>.  P[\<langle>\<rangle>/tr][$tt1\<acute>\<acute>\<acute>/tr\<acute>] ; Q[\<langle>\<rangle>/tr][$tt2\<acute>\<acute>\<acute>/tr\<acute>] \<and> ($tr\<acute> = $tr ^ $tt1\<acute>\<acute>\<acute> ^ $tt2\<acute>\<acute>\<acute>))`"
+  sorry
+
+(*
+proof -
+    have "R2(P);R2(Q) = `( \<exists> tr \<acute>\<acute>\<acute> . 
+      (\<exists> tt1\<acute>\<acute>\<acute> . (P[\<langle>\<rangle>/tr][$tt1\<acute>\<acute>\<acute>/tr\<acute>] \<and> ($tr\<acute>\<acute>\<acute> = $tr ^ $tt1\<acute>\<acute>\<acute>)));
+      (\<exists> tt2\<acute>\<acute>\<acute> . (Q[\<langle>\<rangle>/tr][$tt2\<acute>\<acute>\<acute>/tr\<acute>] \<and> ($tr\<acute> = $tr\<acute>\<acute>\<acute> ^ $tt2\<acute>\<acute>\<acute>)))
+     )`"
+        apply(subst SemiR_extract_variable_ty[of _ _ "tr"])
+        apply(simp_all add:closure assms typing)
+        apply(subst R2_form[of _ "tt1"])
+        apply(simp_all add:closure assms)
+        apply(subst R2_form[of _ "tt2"])
+        apply(simp_all add:closure assms)
+        apply(subst SubstP_ExistsP)
+        apply(simp_all add:closure typing defined unrest)
+        apply(subst SubstP_ExistsP)
+        apply(simp_all add:closure typing defined unrest)
+        apply(simp add:usubst typing defined)
+        apply(simp add: SubstE_PSubstPE SubstE_PSubstPE_dash PSubstPE_Op2PE PSubstPE_PVarPE PSubstPE_PVarPE_different closure typing defined)
+        apply(simp add:usubst typing defined closure)
+        apply(subst SubstP_twice_3) back
+        apply(simp_all add: typing defined closure unrest)
+        apply(subst SubstP_twice_1)
+        apply(simp_all add: typing defined closure unrest)
+        apply (simp add:typing usubst defined closure)
+        apply(subst SubstP_twice_3) back
+        apply (simp_all add:usubst typing defined closure)
+        apply (simp add:unrest typing defined closure)
+   done
+   also have "... = (\<exists>\<^sub>p {tr\<down>\<acute>\<acute>\<acute>} \<union> D\<^sub>2 \<union> {(prime on D\<^sub>1 \<bullet> tt1\<down>\<acute>\<acute>\<acute>)} \<union> {((prime \<circ> prime) on D\<^sub>0 \<bullet> tt2\<down>\<acute>\<acute>\<acute>)} . `(
+      (prime on D\<^sub>1 \<bullet> P)[\<langle>\<rangle>/tr][$(prime on D\<^sub>1 \<bullet> tt1\<acute>\<acute>\<acute>)/tr\<acute>\<acute>] \<and> ($(prime on D\<^sub>1 \<bullet> tr\<acute>\<acute>\<acute>) = $(prime on D\<^sub>1 \<bullet> tr) ^ $(prime on D\<^sub>1 \<bullet> tt1\<acute>\<acute>\<acute>)) \<and>
+      ((prime \<circ> prime) on D\<^sub>0 \<bullet> Q)[\<langle>\<rangle>/tr\<acute>\<acute>][$((prime \<circ> prime) on D\<^sub>0 \<bullet> tt2\<acute>\<acute>\<acute>)/tr\<acute>] \<and> ($((prime \<circ> prime) on D\<^sub>0 \<bullet> tr\<acute>) = $((prime \<circ> prime) on D\<^sub>0 \<bullet> tr\<acute>\<acute>\<acute>) ^ $((prime \<circ> prime) on D\<^sub>0 \<bullet> tt2\<acute>\<acute>\<acute>)))
+`)"
+     apply(subst SemiR_algebraic)
+     apply(simp_all add:closure typing defined unrest urename assms)
+     apply(subst ExistsP_AndP_expand1)
+     defer 
+     apply(subst ExistsP_AndP_expand2)
+     defer 
+     apply(subst ExistsP_union[THEN sym])
+     apply(subst ExistsP_union[THEN sym])
+     apply(subst ExistsP_union[THEN sym])
+     apply(simp add:closure typing defined unrest urename)
+     apply (metis (hide_lams, no_types) AndP_assoc)
+     apply(rule unrest) back back back
+     apply(rule unrest) 
+     apply(rule UNREST_SubstP[of _ _ "{tt1\<down>\<acute>\<acute>\<acute>}" _ "{tt1\<down>\<acute>\<acute>\<acute>}"])
+     apply(simp_all add:typing defined closure unrest urename assms)
+   done
+   also have "... = (\<exists>\<^sub>p {tr\<down>\<acute>\<acute>\<acute>} \<union> D\<^sub>2 \<union> { tt1\<down>\<acute>\<acute>\<acute>} \<union> { tt2\<down>\<acute>\<acute>\<acute>} . `(
+      (prime on D\<^sub>1 \<bullet> P)[\<langle>\<rangle>/tr][$(prime on D\<^sub>1 \<bullet> tt1\<acute>\<acute>\<acute>)/tr\<acute>\<acute>] \<and> ($(prime on D\<^sub>1 \<bullet> tr\<acute>\<acute>\<acute>) = $(prime on D\<^sub>1 \<bullet> tr) ^ $(prime on D\<^sub>1 \<bullet> tt1\<acute>\<acute>\<acute>)) \<and>
+      ((prime \<circ> prime) on D\<^sub>0 \<bullet> Q)[\<langle>\<rangle>/tr\<acute>\<acute>][$((prime \<circ> prime) on D\<^sub>0 \<bullet> tt2\<acute>\<acute>\<acute>)/tr\<acute>] \<and> ($((prime \<circ> prime) on D\<^sub>0 \<bullet> tr\<acute>) = $((prime \<circ> prime) on D\<^sub>0 \<bullet> tr\<acute>\<acute>\<acute>) ^ $((prime \<circ> prime) on D\<^sub>0 \<bullet> tt2\<acute>\<acute>\<acute>)))
+`)"
+  by(simp add:typing defined closure urename)
+   also have "... = `(  \<exists> tt1\<acute>\<acute>\<acute> . \<exists> tt2\<acute>\<acute>\<acute> . \<exists> tr \<acute>\<acute>\<acute> .  
+      (P[\<langle>\<rangle>/tr][$tt1\<acute>\<acute>\<acute>/tr\<acute>] \<and> ($tr\<acute>\<acute>\<acute> = $tr ^ $tt1\<acute>\<acute>\<acute>));
+      (Q[\<langle>\<rangle>/tr][$tt2\<acute>\<acute>\<acute>/tr\<acute>] \<and> ($tr\<acute> = $tr\<acute>\<acute>\<acute> ^ $tt2\<acute>\<acute>\<acute>))
+     )`"
+     apply(subst SemiR_algebraic)
+     apply(rule unrest)
+     apply(subst UNREST_SubstP[of _ _ "D\<^sub>2" _ "D\<^sub>2"])
+     apply(simp_all add:closure typing defined unrest urename assms)
+     apply(simp add:erasure typing defined closure)
+     apply(subst ExistsP_union[THEN sym])
+     apply(subst ExistsP_union[THEN sym])
+     apply(subst ExistsP_union[THEN sym])
+     apply(simp add:closure typing defined urename unrest assms)
+     apply (smt AndP_assoc insert_commute)
+  done
+  also have "... = `(\<exists> tt1\<acute>\<acute>\<acute>. \<exists> tt2\<acute>\<acute>\<acute>. \<exists> tr\<acute>\<acute>\<acute>. ($tr\<acute>\<acute>\<acute> = $tr ^ $tt1\<acute>\<acute>\<acute>) \<and> P[\<langle>\<rangle>/tr][$tt1\<acute>\<acute>\<acute>/tr\<acute>] ; Q[\<langle>\<rangle>/tr][$tt2\<acute>\<acute>\<acute>/tr\<acute>] \<and> ($tr\<acute> = $tr\<acute>\<acute>\<acute> ^ $tt2\<acute>\<acute>\<acute>))`"
+    apply(subst AndP_comm)
+    apply(subst SemiR_AndP_left_precond)
+    defer defer defer 
+    apply(subst SemiR_AndP_right_postcond)
+    defer defer defer 
+    apply(simp_all add:assms unrest closure)
+    sorry (* should be able to do things like SemiR_AndP_left_precond even when not WF_RELATION provided condition is free in dashed variables ? *)
+  also have "... = `(\<exists> tt1\<acute>\<acute>\<acute>. \<exists> tt2\<acute>\<acute>\<acute>.  P[\<langle>\<rangle>/tr][$tt1\<acute>\<acute>\<acute>/tr\<acute>] ; Q[\<langle>\<rangle>/tr][$tt2\<acute>\<acute>\<acute>/tr\<acute>] \<and> (\<exists> tr\<acute>\<acute>\<acute>. ($tr\<acute> = $tr\<acute>\<acute>\<acute> ^ $tt2\<acute>\<acute>\<acute>) \<and> ($tr\<acute>\<acute>\<acute> = $tr ^ $tt1\<acute>\<acute>\<acute>)))`"
+    apply(subst AndP_comm)
+    apply(subst AndP_assoc[THEN sym])
+    apply(subst ExistsP_AndP_expand2[THEN sym])
+    apply(simp_all add:unrest typing defined closure assms)
+    sorry (*unrest problem *)
+  also have "... = `(\<exists> tt1\<acute>\<acute>\<acute>. \<exists> tt2\<acute>\<acute>\<acute>.  P[\<langle>\<rangle>/tr][$tt1\<acute>\<acute>\<acute>/tr\<acute>] ; Q[\<langle>\<rangle>/tr][$tt2\<acute>\<acute>\<acute>/tr\<acute>] \<and> ($tr\<acute> = $tr ^ $tt1\<acute>\<acute>\<acute> ^ $tt2\<acute>\<acute>\<acute>))`"
+    proof -
+      have  "`(\<exists> tr\<acute>\<acute>\<acute>. ($tr\<acute> = $tr\<acute>\<acute>\<acute> ^ $tt2\<acute>\<acute>\<acute>) \<and> ($tr\<acute>\<acute>\<acute> = $tr ^ $tt1\<acute>\<acute>\<acute>))` = `($tr\<acute> = $tr ^ $tt1\<acute>\<acute>\<acute> ^ $tt2\<acute>\<acute>\<acute>)`" 
+        apply(simp add:erasure typing defined closure)
+        apply(subst ExistsP_one_point)
+        apply(simp_all add:unrest typing defined closure)
+        apply(subst SubstP_EqualP)
+        apply(simp add:usubst typing defined closure append_assoc)
+      done
+      thus ?thesis 
+        by metis
+    qed
+  finally show ?thesis
+    ..
+qed
+*)
+
+lemma R2_SemiR_distribute:
+  assumes "P \<in> WF_RELATION" "Q \<in> WF_RELATION"
+  shows "R2(P);R2(Q) is R2"
+proof-
+  have "R2(R2(P);R2(Q)) =  `(\<exists> tt1\<acute>\<acute>\<acute> . \<exists> tt2\<acute>\<acute>\<acute> . \<exists> tt\<acute>\<acute>\<acute> . P[\<langle>\<rangle>/tr][$tt1\<acute>\<acute>\<acute>/tr\<acute>] ; Q[\<langle>\<rangle>/tr][$tt2\<acute>\<acute>\<acute>/tr\<acute>] \<and> ($tt\<acute>\<acute>\<acute> = $tt1\<acute>\<acute>\<acute> ^ $tt2\<acute>\<acute>\<acute>) \<and> ($tr\<acute> = $tr ^ $tt\<acute>\<acute>\<acute>))`"
+   apply(subst R2_form[of _ "tt"])
+   apply(simp_all add:closure assms typing defined)
+   apply(subst R2_SemiR_form)
+   apply(simp_all add: assms)
+   apply(subst SubstP_ExistsP)
+   apply(simp_all add:unrest closure typing defined)
+   apply(subst SubstP_ExistsP)
+   apply(simp_all add:unrest closure typing defined)
+   apply(subst SubstP_AndP)
+   apply(subst SubstP_SemiR_left)
+   apply(simp_all add:unrest closure typing defined)
+   apply(subst SubstP_twice_2) back
+   apply(simp_all add:unrest closure typing defined)
+   apply(subst SubstP_EqualP)
+   apply(subst SubstP_ExistsP)
+   apply(simp_all add:unrest closure typing defined)
+   apply(subst SubstP_ExistsP)
+   apply(simp_all add:unrest closure typing defined)
+   apply(subst SubstP_AndP)
+   apply(subst SubstP_SemiR_right)
+   apply(simp_all add:unrest closure typing defined)
+   apply(subst SubstP_twice_1)
+   apply(simp_all add:unrest closure typing defined)
+   apply(subst SubstP_EqualP)
+   apply(simp add:usubst typing defined closure)
+   apply(subst ExistsP_AndP_expand1)
+   apply(simp add:unrest closure typing defined)
+   apply(subst ExistsP_AndP_expand1)
+   apply(simp add:unrest closure typing defined)
+   apply(subst AndP_assoc[THEN sym])
+   apply(simp add: ExistsP_union[THEN sym])
+   apply (metis insert_commute)
+   done
+   also have "... = `(\<exists> tt1\<acute>\<acute>\<acute> . \<exists> tt2\<acute>\<acute>\<acute> . P[\<langle>\<rangle>/tr][$tt1\<acute>\<acute>\<acute>/tr\<acute>] ; Q[\<langle>\<rangle>/tr][$tt2\<acute>\<acute>\<acute>/tr\<acute>] \<and> (\<exists> tt\<acute>\<acute>\<acute> . ($tt\<acute>\<acute>\<acute> = $tt1\<acute>\<acute>\<acute> ^ $tt2\<acute>\<acute>\<acute>) \<and> ($tr\<acute> = $tr ^ $tt\<acute>\<acute>\<acute>)))`"
+   apply(subst ExistsP_AndP_expand2[THEN sym])
+   apply(simp_all add:unrest closure typing defined)
+   sorry (*UNREST problem *)
+   also have "... = `(\<exists> tt1\<acute>\<acute>\<acute> . \<exists> tt2\<acute>\<acute>\<acute> . P[\<langle>\<rangle>/tr][$tt1\<acute>\<acute>\<acute>/tr\<acute>] ; Q[\<langle>\<rangle>/tr][$tt2\<acute>\<acute>\<acute>/tr\<acute>] \<and> ($tr\<acute> = $tr ^ $tt1\<acute>\<acute>\<acute> ^ $tt2\<acute>\<acute>\<acute>))`"
+   apply(subst AndP_comm) back
+   apply(simp add:PVarPE_erasure typing defined closure)
+   apply(subst ExistsP_one_point[of _ "tt\<down>\<acute>\<acute>\<acute>"])
+   apply(simp add:closure typing defined unrest erasure)
+   apply(auto intro!:unrest closure typing simp add:typing closure)[1]
+   apply(subst SubstP_EqualP)
+   apply(simp add:usubst typing defined closure)
+   done 
+    also have "... = R2(P);R2(Q)" by(subst R2_SemiR_form,simp_all add:assms)
+    finally show ?thesis by(simp add:is_healthy_def)
+qed
+
+lemma R2_SemiR_closure: 
+assumes "P is R2" "Q is R2" "P \<in> WF_RELATION" "Q \<in> WF_RELATION"
+shows "P;Q is R2"
+by (metis Healthy_simp R2_SemiR_distribute assms)
+
 lemma R2_sequential_composition: 
   assumes "P \<in> WF_RELATION" "Q \<in> WF_RELATION"
   shows "`R2(P);R2(Q)` = `R2(P ; R2(Q))`"
 proof -
-have "`R2(P;R2(Q))` = `R2(\<exists> tr\<acute>\<acute>\<acute> . (P[$tr\<acute>\<acute>\<acute>/tr\<acute>]);(R2(Q)[$tr\<acute>\<acute>\<acute>/tr]))`"
-  apply(subst SemiR_extract_variable[where x="tr \<down>"])
-  apply (metis assms(1))
-  apply (metis R2_rel_closure assms(2))
-  apply (metis MkPlain_UNDASHED PVAR_VAR_MkPVAR)
-  apply (simp add:closure typing defined erasure)
-  done
-also have "... = `R1(
-
-(\<exists> tr\<acute>\<acute>\<acute> . P[$tr\<acute>\<acute>\<acute>/tr\<acute>];(Q[\<langle>\<rangle>/tr][($tr\<acute> - $tr)/tr\<acute>] \<and>  ($tr \<le> $tr\<acute>))[$tr\<acute>\<acute>\<acute>/tr])
-
-[\<langle>\<rangle>/tr][($tr\<acute> - $tr)/tr\<acute>]
-
-)`"
-  by(simp add:R2_def R1_def R2s_def)
-also have "... = `R1(\<exists> tr\<acute>\<acute>\<acute> . (P[$tr\<acute>\<acute>\<acute>/tr\<acute>];(Q[\<langle>\<rangle>/tr][($tr\<acute> - $tr)/tr\<acute>] \<and>  ($tr \<le> $tr\<acute>))[$tr\<acute>\<acute>\<acute>/tr])[\<langle>\<rangle>/tr][($tr\<acute> - $tr)/tr\<acute>])`"
-  apply(subst SubstP_ExistsP)
-  apply(simp_all add:unrest typing defined closure)
-  apply(subst SubstP_ExistsP)
-  apply(simp_all add:unrest typing defined closure)
-  done
-also have "... = `R1(\<exists> tr\<acute>\<acute>\<acute> . (P[\<langle>\<rangle>/tr][$tr\<acute>\<acute>\<acute>/tr\<acute>];(Q[\<langle>\<rangle>/tr][(($tr\<acute> - $tr) - $tr\<acute>\<acute>\<acute>)/tr\<acute>] \<and>  ($tr\<acute>\<acute>\<acute> \<le> ($tr\<acute> - $tr)))))`"
-   apply(subst SubstP_SemiR_left[of "tr \<down>"])
-   apply (metis MkPlain_UNDASHED PVAR_VAR_MkPVAR)
-   apply(simp_all add:unrest typing defined closure)
-   sorry (*distributing substitution through SemiR *)
-also have "... = `R1(\<exists> tr\<acute>\<acute>\<acute>\<acute> . \<exists> tr\<acute>\<acute>\<acute> . $tr\<acute>\<acute>\<acute>\<acute> = $tr^$tr\<acute>\<acute>\<acute> \<and> (P[\<langle>\<rangle>/tr][($tr\<acute>\<acute>\<acute>\<acute> - $tr)/tr\<acute>];(Q[\<langle>\<rangle>/tr][(($tr\<acute> - $tr) - ($tr\<acute>\<acute>\<acute>\<acute> - $tr))/tr\<acute>] \<and>  (($tr\<acute>\<acute>\<acute>\<acute> - $tr) \<le> ($tr\<acute> - $tr)))))`" sorry (*introduce fresh quantifier *)
-also have "... = `R1(\<exists> tr\<acute>\<acute>\<acute>\<acute> . (P[\<langle>\<rangle>/tr][($tr\<acute>\<acute>\<acute>\<acute> - $tr)/tr\<acute>];(Q[\<langle>\<rangle>/tr][(($tr\<acute> - $tr) - ($tr\<acute>\<acute>\<acute>\<acute> - $tr))/tr\<acute>] \<and>  (($tr\<acute>\<acute>\<acute>\<acute> - $tr) \<le> ($tr\<acute> - $tr)))))`" sorry (*remove old quantifier *)
-also have "... = `R1(\<exists> tr\<acute>\<acute>\<acute>\<acute> . (P[\<langle>\<rangle>/tr][($tr\<acute> - $tr)/tr\<acute>][$tr\<acute>\<acute>\<acute>\<acute>/tr\<acute>];(Q[\<langle>\<rangle>/tr][($tr\<acute> - $tr)/tr\<acute>][$tr\<acute>\<acute>\<acute>\<acute>/tr\<acute>] \<and>  ($tr \<le> $tr\<acute>\<acute>\<acute>\<acute>) \<and> ($tr\<acute>\<acute>\<acute>\<acute> \<le> $tr\<acute>))))`" sorry (*resolving substitutions *)
-also have "... = `R1(\<exists> tr\<acute>\<acute>\<acute>\<acute> . ((P[\<langle>\<rangle>/tr][($tr\<acute> - $tr)/tr\<acute>][$tr\<acute>\<acute>\<acute>\<acute>/tr\<acute>] \<and> ($tr \<le> $tr\<acute>)[$tr\<acute>\<acute>\<acute>\<acute>/tr\<acute>]);(Q[\<langle>\<rangle>/tr][($tr\<acute> - $tr)/tr\<acute>][$tr\<acute>\<acute>\<acute>\<acute>/tr] \<and> ($tr \<le> $tr\<acute>)[$tr\<acute>\<acute>\<acute>\<acute>/tr])))`" sorry (*resolving substitutions *)
-also have "... = `R1(\<exists> tr\<acute>\<acute>\<acute>\<acute> . ((P[\<langle>\<rangle>/tr][($tr\<acute> - $tr)/tr\<acute>] \<and> ($tr \<le> $tr\<acute>))[$tr\<acute>\<acute>\<acute>\<acute>/tr\<acute>];(Q[\<langle>\<rangle>/tr][($tr\<acute> - $tr)/tr\<acute>] \<and> ($tr \<le> $tr\<acute>))[$tr\<acute>\<acute>\<acute>\<acute>/tr]))`" 
-  by(simp add:usubst)
-also have "... = `R1(\<exists> tr\<acute>\<acute>\<acute> . ((P[\<langle>\<rangle>/tr][($tr\<acute> - $tr)/tr\<acute>] \<and> ($tr \<le> $tr\<acute>))[$tr\<acute>\<acute>\<acute>/tr\<acute>];(Q[\<langle>\<rangle>/tr][($tr\<acute> - $tr)/tr\<acute>] \<and> ($tr \<le> $tr\<acute>))[$tr\<acute>\<acute>\<acute>/tr]))`" sorry (*rename quantifier*)
-also have "... = `R1(\<exists> tr\<acute>\<acute>\<acute> . (R2(P)[$tr\<acute>\<acute>\<acute>/tr\<acute>];R2(Q)[$tr\<acute>\<acute>\<acute>/tr]))`" 
-  by(simp add:R1_def R2_def R2s_def)
-also have "... = `R1(R2(P);R2(Q))`"
-  apply(subst SemiR_extract_variable[where x="tr \<down>"]) back
-  apply (metis R2_rel_closure assms(1))
-  apply (metis R2_rel_closure assms(2))
-  apply (metis MkPlain_UNDASHED PVAR_VAR_MkPVAR)
-  apply (simp add:closure typing defined erasure)
-  done
-also have "... = `R2(P);R2(Q)`"
-  proof -
-  have "`R2(P);R2(Q)` is R1" 
-    by(subst R1_SemiR_closure, simp_all add: assms R2_rel_closure, simp_all add:R2_def is_healthy_def R1_idempotent)
-  thus ?thesis 
-    by (metis Healthy_simp)
-  qed
-finally show ?thesis by simp 
+  have 1: "`R2(P);R2(Q)` = `R2(R2(P);R2(Q))`"  
+    by (metis R2_SemiR_distribute assms is_healthy_def)
+  have 2: "R2(P);R2(Q)  = (\<exists>\<^sub>p {tt\<down>\<acute>\<acute>\<acute>,tt1\<down>\<acute>\<acute>\<acute>,tt2\<down>\<acute>\<acute>\<acute>} . `(P[\<langle>\<rangle>/tr][$tt1\<acute>\<acute>\<acute>/tr\<acute>] ; Q[\<langle>\<rangle>/tr][$tt2\<acute>\<acute>\<acute>/tr\<acute>] \<and> ($tt\<acute>\<acute>\<acute> = $tt1\<acute>\<acute>\<acute> ^ $tt2\<acute>\<acute>\<acute>) \<and> ($tr\<acute> = $tr ^ $tt\<acute>\<acute>\<acute>))`)"
+    apply(subst 1)
+    apply(subst R2_form[of _ "tt"])
+    apply(metis assms closure)
+    apply (metis pvaux_MkPVAR)
+    apply(subst R2_SemiR_form)
+    apply(simp_all add:assms)
+    apply(subst SubstP_ExistsP)
+    apply(simp_all add:closure typing defined unrest)
+    apply(subst SubstP_ExistsP)
+    apply(simp_all add:closure typing defined unrest)
+    apply(subst SubstP_AndP)
+    apply(subst SubstP_SemiR_left)
+    apply(simp_all add:closure typing defined unrest)
+    apply(subst SubstP_twice_2) back
+    apply(simp_all add:closure typing defined unrest)
+    apply(subst SubstP_EqualP)
+    apply(subst SubstP_ExistsP)
+    apply(simp_all add:closure typing defined unrest)
+    apply(subst SubstP_ExistsP)
+    apply(simp_all add:closure typing defined unrest)
+    apply(subst SubstP_AndP)
+    apply(subst SubstP_SemiR_right)
+    apply(simp_all add:closure typing defined unrest)
+    apply(subst SubstP_twice_1)
+    apply(simp_all add:closure typing defined unrest)
+    apply(subst SubstP_EqualP)
+    apply(simp add:usubst typing defined closure)
+    apply(subst ExistsP_AndP_expand1)
+    apply(simp_all add:closure typing defined unrest)
+    apply(subst ExistsP_AndP_expand1)
+    apply(simp_all add:closure typing defined unrest)
+    apply(subst ExistsP_union[THEN sym])
+    apply(subst ExistsP_union[THEN sym])
+    apply (smt AndP_assoc Un_insert_left sup_bot_left)
+    done
+  have "R2(P ; R2(Q)) =  (\<exists>\<^sub>p {tt\<down>\<acute>\<acute>\<acute>} . (\<exists>\<^sub>p {tr\<down>\<acute>\<acute>\<acute>} . 
+    `P[\<langle>\<rangle>/tr][$tr\<acute>\<acute>\<acute>/tr\<acute>] ; (\<exists> tt2\<acute>\<acute>\<acute> . Q[\<langle>\<rangle>/tr][$tt2\<acute>\<acute>\<acute>/tr\<acute>] \<and> ($tt\<acute>\<acute>\<acute> = $tr\<acute>\<acute>\<acute> ^ $tt2\<acute>\<acute>\<acute>)) \<and>
+     ($tr\<acute> = $tr ^ $tt\<acute>\<acute>\<acute>)`))"
+    apply(subst R2_form[of _ "tt"])
+    apply(metis assms closure)
+    apply (metis pvaux_MkPVAR)
+    apply(subst SemiR_extract_variable_ty[of _ _ "tr "])
+    apply(simp_all add:assms closure typing)
+    apply(subst SubstP_ExistsP)
+    apply(simp_all add:typing closure unrest defined)
+    apply(subst SubstP_SemiR_left)
+    apply(simp_all add:typing closure unrest defined)
+    apply(subst SubstP_twice_3)
+    apply(simp_all add:typing closure unrest defined)
+    apply(subst SubstP_ExistsP)
+    apply(simp_all add:typing closure unrest defined)
+    apply(subst SubstP_SemiR_right)
+    apply(simp_all add:typing closure unrest defined)
+    apply(simp add:erasure typing defined closure)
+(*    apply(simp add:usubst typing defined closure assms) *)
+    apply(subst R2_form[of _ "tt2"])
+    apply(metis assms(2))
+    apply (metis pvaux_MkPVAR)
+    apply(subst SubstP_ExistsP)
+    apply(simp_all add:typing closure unrest defined)
+    apply(subst SubstP_AndP)
+    apply(subst SubstP_twice_2) back back
+    apply(simp_all add:typing closure unrest defined)
+    apply(subst SubstP_ExistsP)
+    apply(simp_all add:typing closure unrest defined)
+    apply(subst SubstP_AndP)
+    apply(subst SubstP_twice_1)
+    apply(simp_all add:typing closure unrest defined)
+    apply(subst SubstP_EqualP)
+    apply(subst SubstP_EqualP)
+    sorry
+(*
+    apply(simp add:usubst typing defined closure)
+    apply(subst ExistsP_AndP_expand1)
+    apply(simp_all add:typing defined closure unrest)
+    done
+*)
+  also have "... = (\<exists>\<^sub>p D\<^sub>2 \<union> {tt\<down>\<acute>\<acute>\<acute>,tr\<down>\<acute>\<acute>\<acute>,tt2\<down>\<acute>\<acute>\<acute>} .
+     `(prime on D\<^sub>1 \<bullet> P)[\<langle>\<rangle>/tr][$(prime on D\<^sub>1 \<bullet> tr\<acute>\<acute>\<acute>)/tr\<acute>\<acute>] \<and>
+      ((prime \<circ> prime) on D\<^sub>0 \<bullet> Q)[\<langle>\<rangle>/tr\<acute>\<acute>][$((prime \<circ> prime) on D\<^sub>0 \<bullet> tt2\<acute>\<acute>\<acute>)/tr\<acute>] \<and> ($((prime \<circ> prime) on D\<^sub>0 \<bullet> tt\<acute>\<acute>\<acute>) = $((prime \<circ> prime) on D\<^sub>0 \<bullet> tr\<acute>\<acute>\<acute>) ^ $((prime \<circ> prime) on D\<^sub>0 \<bullet> tt2\<acute>\<acute>\<acute>)) \<and>
+     ($tr\<acute> = $tr ^ $tt\<acute>\<acute>\<acute>)`)"
+     apply(subst SemiR_algebraic)
+     apply(rule UNREST_SubstP[of _ _ "D\<^sub>2" _ "D\<^sub>2"])
+     apply(simp_all add:closure typing defined unrest)
+     apply(rule UNREST_SubstP[of _ _ "D\<^sub>2" _ "D\<^sub>2"])
+     apply(simp_all add:closure typing defined unrest assms)
+     apply(subst ExistsP_AndP_expand1)
+     apply(simp add:typing unrest defined closure assms)
+     apply (simp add:urename closure typing defined assms)
+(*    apply(rule unrest)
+     apply(rule unrest)
+     apply(simp add:typing defined closure)
+     apply(rule unrest)
+     apply(utp_pred_auto_tac)
+     apply(rule unrest)
+     apply(simp add:typing defined closure)
+     apply(rule unrest)
+     apply(rule unrest)
+     apply(utp_pred_auto_tac)
+     apply(rule unrest)
+     apply(utp_pred_auto_tac)
+     apply (metis dash_DASHED_TWICE_elim undash_dash undash_eq_dash_contra1)
+     apply(subst ExistsP_AndP_expand1)
+     apply(rule unrest) back back
+     apply(simp add:erasure typing defined closure)
+     apply(rule unrest)
+     apply(utp_pred_auto_tac)
+     apply(rule unrest)
+     apply(simp add:typing defined closure)
+     apply(rule unrest)
+     apply(rule unrest)
+     apply(utp_pred_auto_tac)
+     apply(rule unrest)
+     apply(utp_pred_auto_tac)
+     apply(subst ExistsP_union[THEN sym])
+     apply(subst ExistsP_union[THEN sym])
+     apply(subst ExistsP_union[THEN sym])
+     apply (smt AndP_assoc Un_insert_left Un_insert_right sup_bot_left sup_bot_right)*)
+     sorry (* more little bits *)
+also have "... = (\<exists>\<^sub>p {tt\<down>\<acute>\<acute>\<acute>,tr\<down>\<acute>\<acute>\<acute>,tt2\<down>\<acute>\<acute>\<acute>} .  
+    `P[\<langle>\<rangle>/tr][$tr\<acute>\<acute>\<acute>/tr\<acute>] ; (Q[\<langle>\<rangle>/tr][$tt2\<acute>\<acute>\<acute>/tr\<acute>] \<and> ($tt\<acute>\<acute>\<acute> = $tr\<acute>\<acute>\<acute> ^ $tt2\<acute>\<acute>\<acute>)) \<and>
+     ($tr\<acute> = $tr ^ $tt\<acute>\<acute>\<acute>)`)"
+     apply(subst SemiR_algebraic)
+     apply(rule UNREST_SubstP[of _ _ "D\<^sub>2" _ "D\<^sub>2"])
+     apply(simp_all add:typing defined closure unrest)
+     apply(rule UNREST_SubstP[of _ _ "D\<^sub>2" _ "D\<^sub>2"])
+     apply(simp_all add:typing defined closure unrest assms)
+     apply(simp add:erasure typing defined closure)
+(*
+     apply(rule unrest)
+     apply(utp_pred_auto_tac)
+     apply (metis DASHED_dash_not_DASHED MkPlainP_UNDASHED PVAR_VAR_PUNDASHED_UNDASHED UNDASHED_dash_DASHED dash_DASHED_TWICE_elim) 
+     apply(rule unrest)
+     apply(rule UNREST_SubstP[of _ _ "D\<^sub>2" _ "D\<^sub>2"])
+     apply(simp_all add:typing defined closure unrest assms)
+     apply(simp add:erasure typing defined closure)
+     apply(rule unrest)
+     apply(utp_pred_auto_tac)
+     apply (metis DASHED_dash_not_DASHED MkPlainP_UNDASHED PVAR_VAR_PUNDASHED_UNDASHED UNDASHED_dash_DASHED dash_DASHED_TWICE_elim) 
+     apply(rule unrest)
+     apply(simp add:erasure typing defined closure)
+     apply(rule unrest)
+     apply(utp_pred_auto_tac)
+     apply (metis DASHED_dash_not_DASHED MkPlainP_UNDASHED PVAR_VAR_PUNDASHED_UNDASHED UNDASHED_dash_DASHED dash_DASHED_TWICE_elim) 
+     apply(rule unrest)
+     apply(simp add:typing defined closure)
+     apply(rule unrest)
+     apply(rule unrest)
+     apply(utp_pred_auto_tac)
+     apply (metis DASHED_dash_not_DASHED MkPlainP_UNDASHED PVAR_VAR_PUNDASHED_UNDASHED UNDASHED_dash_DASHED dash_DASHED_TWICE_elim) 
+     apply(rule unrest)
+     apply(utp_pred_auto_tac)
+     apply (metis DASHED_dash_not_DASHED MkPlainP_UNDASHED PVAR_VAR_PUNDASHED_UNDASHED UNDASHED_dash_DASHED dash_DASHED_TWICE_elim) 
+     apply (subst ExistsP_AndP_expand1)
+     apply(rule unrest)
+     apply(simp add:erasure typing defined closure)
+     apply(rule unrest)
+     apply(utp_pred_auto_tac)
+     apply(rule unrest)
+     apply(simp add:typing defined closure)
+     apply(rule unrest)
+     apply(rule unrest)
+     apply(utp_pred_auto_tac)
+     apply(rule unrest)
+     apply(utp_pred_auto_tac)
+     apply (metis DASHED_dash_not_DASHED MkPlainP_UNDASHED PVAR_VAR_PUNDASHED_UNDASHED UNDASHED_dash_DASHED dash_DASHED_TWICE_elim) 
+     apply(subst ExistsP_union[THEN sym])
+     apply(simp add:typing defined closure urename)
+     apply (smt AndP_assoc)
+     done *)
+     sorry
+  also have "... = (\<exists>\<^sub>p {tt\<down>\<acute>\<acute>\<acute>,tr\<down>\<acute>\<acute>\<acute>,tt2\<down>\<acute>\<acute>\<acute>} .  
+    `P[\<langle>\<rangle>/tr][$tr\<acute>\<acute>\<acute>/tr\<acute>] ; Q[\<langle>\<rangle>/tr][$tt2\<acute>\<acute>\<acute>/tr\<acute>] \<and> 
+      ($tt\<acute>\<acute>\<acute> = $tr\<acute>\<acute>\<acute> ^ $tt2\<acute>\<acute>\<acute>) \<and> ($tr\<acute> = $tr ^ $tt\<acute>\<acute>\<acute>)`)"
+      apply(subst SemiR_AndP_right_postcond)
+      defer defer defer 
+      apply(utp_pred_auto_tac)
+     sorry (*SemiR_AndP_right_postcond on non WF_RELATION *)
+   finally have 3: "R2(P;R2(Q)) = (\<exists>\<^sub>p {tt\<down>\<acute>\<acute>\<acute>,tr\<down>\<acute>\<acute>\<acute>,tt2\<down>\<acute>\<acute>\<acute>} .  
+    `P[\<langle>\<rangle>/tr][$tr\<acute>\<acute>\<acute>/tr\<acute>] ; Q[\<langle>\<rangle>/tr][$tt2\<acute>\<acute>\<acute>/tr\<acute>] \<and> ($tt\<acute>\<acute>\<acute> = $tr\<acute>\<acute>\<acute> ^ $tt2\<acute>\<acute>\<acute>) \<and> ($tr\<acute> = $tr ^ $tt\<acute>\<acute>\<acute>)`)"
+      ..
+   show ?thesis 
+      apply(subst 2) 
+      apply(subst 3)
+      sorry (*renaming a quantified variable *)
 qed
 
 lemma R2_composition: 
@@ -621,22 +721,6 @@ lemma R2_composition:
   shows "R2(P ; R2(Q)) = R2(P) ; R2(Q)"
 by (metis R2_sequential_composition assms(1) assms(2))
    
-(* L8 R2-sequence-closure *)
-
-lemma R2_SemiR_closure: 
-assumes "P is R2" "Q is R2" "P \<in> WF_RELATION" "Q \<in> WF_RELATION"
-shows "`P;Q` is R2"
-proof -
-  have "`R2(P;Q)`=`R2(P;R2(Q))`"
-    by(metis assms(2) is_healthy_def)
-  also have "... = R2(P);R2(Q)"
-    by(metis R2_composition assms(3) assms(4))
-  also have "... = P ; Q"
-    by(metis assms is_healthy_def)
-  finally show ?thesis 
-    by (simp add:is_healthy_def)
-qed
-*)
 (* L10 R2-wait-okay' *)
 
 lemma R2_wait_true: "(R2(P))\<^sub>t = R2(P\<^sub>t)"
@@ -671,135 +755,6 @@ lemma R2_wait_false: "(R2(P))\<^sub>f = R2(P\<^sub>f)"
   apply(simp add:unrest closure typing defined)
   done
 
-lemma R2_okay'_true: "(R2(P))\<^sup>t = R2(P\<^sup>t)"  
-  apply(simp add:R2_def R1_okay'_false R2s_def)
-  apply(subst SubstP_twice_3) back
-  apply(simp_all)
-  apply(utp_pred_auto_tac)
-  apply(utp_pred_auto_tac)
-  apply(simp_all add:usubst typing defined closure)
-  apply(simp add:unrest closure typing defined)
-  apply(subst SubstP_twice_3) back back
-  apply(simp_all)
-  apply(utp_pred_auto_tac)
-  apply(utp_pred_auto_tac)
-  apply(simp_all add:usubst typing defined closure)
-  apply(simp add:unrest closure typing defined)
-  apply (metis (hide_lams, no_types) PVAR_VAR_pvdash R1_okay'_true)
-  done
-
-lemma R2_okay'_false: "(R2(P))\<^sup>f = R2(P\<^sup>f)"
-  apply(simp add:R2_def R1_okay'_false R2s_def)
-  apply(subst SubstP_twice_3) back
-  apply(simp_all)
-  apply(utp_pred_auto_tac)
-  apply(utp_pred_auto_tac)
-  apply(simp_all add:usubst typing defined closure)
-  apply(simp add:unrest closure typing defined)
-  apply(subst SubstP_twice_3) back back
-  apply(simp_all)
-  apply(utp_pred_auto_tac)
-  apply(utp_pred_auto_tac)
-  apply(simp_all add:usubst typing defined closure)
-  apply(simp add:unrest closure typing defined)
-  apply (metis (hide_lams, no_types) PVAR_VAR_pvdash R1_okay'_false)
-  done
-
-lemma R2_okay_true: "`(R2(P))[true/okay]` = `R2(P[true/okay])`"  
-  apply(simp add:R2_def R1_def usubst typing defined closure)
-  apply(simp add:R2s_def)
-  apply(subst SubstP_twice_3) back
-  apply(simp_all)
-  apply(utp_pred_auto_tac)
-  apply(utp_pred_auto_tac)
-  apply(simp_all add:usubst typing defined closure)
-  apply(simp add:unrest closure typing defined)
-  apply(subst SubstP_twice_3) back back
-  apply(simp_all)
-  apply(utp_pred_auto_tac)
-  apply(utp_pred_auto_tac)
-  apply(simp_all add:usubst typing defined closure)
-  apply(simp add:unrest closure typing defined)
-  done
-
-lemma R2_okay_false: "`(R2(P))[false/okay]` = `R2(P[false/okay])`"  
-  apply(simp add:R2_def R1_def usubst typing defined closure)
-  apply(simp add:R2s_def)
-  apply(subst SubstP_twice_3) back
-  apply(simp_all)
-  apply(utp_pred_auto_tac)
-  apply(utp_pred_auto_tac)
-  apply(simp_all add:usubst typing defined closure)
-  apply(simp add:unrest closure typing defined)
-  apply(subst SubstP_twice_3) back back
-  apply(simp_all)
-  apply(utp_pred_auto_tac)
-  apply(utp_pred_auto_tac)
-  apply(simp_all add:usubst typing defined closure)
-  apply(simp add:unrest closure typing defined)
-  done
-
-(* L11 J-R2 *)
-
-lemma J_is_R2: 
-  "J is R2"
-
-proof -
-  have "R2 J = `R1 ((ok \<Rightarrow> ok') \<and> (($tr\<acute> - $tr) = \<langle>\<rangle>) \<and> II\<^bsub>REL_VAR - {okay\<down>, okay\<down>\<acute>} - {tr\<down>, tr\<down>\<acute>}\<^esub>)`"
-    apply (simp add:J_pred_def)
-    apply (subst SkipRA_unfold[of "tr \<down>"])
-    apply (simp_all)
-    apply (metis MkPlain_UNDASHED PVAR_VAR_MkPVAR)
-    apply (metis MkPlain_UNDASHED PVAR_VAR_MkPVAR UNDASHED_dash_DASHED)
-    apply (metis MkPlain_UNDASHED PVAR_VAR_MkPVAR)
-    apply (utp_pred_auto_tac)
-    apply (simp add:is_healthy_def R2_def R2s_def)
-    apply (simp add:usubst typing defined closure)
-    done
-  also have "... = `(ok \<Rightarrow> ok') \<and> R1(($tr\<acute> - $tr) = \<langle>\<rangle>) \<and> II\<^bsub>REL_VAR - {okay\<down>, okay\<down>\<acute>} - {tr\<down>, tr\<down>\<acute>}\<^esub>`"
-    by (utp_pred_auto_tac)
-  also have "... = `(ok \<Rightarrow> ok') \<and> ($tr\<acute> = $tr) \<and> II\<^bsub>REL_VAR - {okay\<down>, okay\<down>\<acute>} - {tr\<down>, tr\<down>\<acute>}\<^esub>`"
-    by (simp add:R1_def tr_prefix_as_nil)
-  also have "... = J"
-    apply(simp add:J_pred_def)
-    apply(subst SkipRA_unfold[of "tr \<down>"]) back
-    apply(simp_all)
-    apply (metis MkPlain_UNDASHED PVAR_VAR_MkPVAR)
-    apply (metis MkPlain_UNDASHED PVAR_VAR_MkPVAR UNDASHED_dash_DASHED)
-    apply (metis MkPlain_UNDASHED PVAR_VAR_MkPVAR)
-    apply (utp_pred_auto_tac)
-    apply(simp add:closure typing defined erasure)
-    done
-  finally show ?thesis 
-    by (simp add:is_healthy_def)
-qed
-
-(* L12 commutativity-R2-H1 *)
-(*No longer holds in original form since R2 has R1 like properties *)
-
-lemma H1_R2s_commute: "H1 (R2s P) = R2s (H1 P)"
-  by(simp add:H1_def R2s_def usubst typing defined closure)
-
-(* L13 commutativity R2-H2 *)
-(*
-lemma H2_R2_commute: 
-  assumes "P \<in> WF_RELATION"
-  shows "H2 (R2 P) = R2 (H2 P)" 
-proof -
-  have "H2 (R2 P) = (R2 P);(R2 J)" 
-    by(metis H2_def J_is_R2 is_healthy_def)
-  also have "... = R2 (P ; (R2 J))"
-    apply(subst R2_composition)
-    apply (metis assms)
-    apply (metis J_closure)
-    apply (simp)
-    done
-  also have "... = R2 (P ; J) " 
-    by(metis J_is_R2 is_healthy_def)
-  finally show ?thesis 
-    by(simp add:H2_def)
-qed
-*)
 (* L14 commutativity R2-R1 *)
 
 lemma R1_R2_commute: 
@@ -811,37 +766,28 @@ by (simp add:R2_def R1_idempotent R2s_destroys_R1)
 lemma R2_monotonic: "P \<sqsubseteq> Q \<Longrightarrow> R2(P) \<sqsubseteq> R2(Q)" 
   by utp_pred_tac
 
-lemma SkipRA_is_R2 : "`R2(II\<^bsub>REL_VAR - OKAY\<^esub>)` = `II\<^bsub>REL_VAR - OKAY\<^esub>`"
+lemma SkipRA_is_R2 : "`R2(II)` = `II`"
 proof -
-  have "`R2(II\<^bsub>REL_VAR - OKAY\<^esub>)` = `(($tr\<acute> - $tr) = \<langle>\<rangle> \<and> II\<^bsub>REL_VAR - OKAY - TR\<^esub>) \<and> ($tr \<le> $tr\<acute>)`"
+  have "`R2(II\<^bsub>REL_VAR\<^esub>)` = `(($tr\<acute> - $tr) = \<langle>\<rangle> \<and> II\<^bsub>REL_VAR - TR\<^esub>) \<and> ($tr \<le> $tr\<acute>)`"
     apply (simp add:R1_def R2_def R2s_def)
     apply (subst SkipRA_unfold[of "tr\<down>"])
     apply (auto simp add:closure)
     apply (simp add:usubst closure typing defined)
   done
 
-  also have "... = `(($tr\<acute> - $tr) = \<langle>\<rangle> \<and> ($tr \<le> $tr\<acute>)) \<and> II\<^bsub>REL_VAR - OKAY - TR\<^esub>`"
+  also have "... = `(($tr\<acute> - $tr) = \<langle>\<rangle> \<and> ($tr \<le> $tr\<acute>)) \<and> II\<^bsub>REL_VAR - TR\<^esub>`"
     by (metis (hide_lams, no_types) AndP_assoc AndP_comm)
 
-  also have "... = `$tr\<acute> = $tr \<and> II\<^bsub>REL_VAR - OKAY - TR\<^esub>`"
+  also have "... = `$tr\<acute> = $tr \<and> II\<^bsub>REL_VAR - TR\<^esub>`"
     by (metis EqualP_sym tr_prefix_as_nil)
 
-  also have "... = `II\<^bsub>REL_VAR - OKAY\<^esub>`"
+  also have "... = `II\<^bsub>REL_VAR\<^esub>`"
     apply (subst SkipRA_unfold[of "tr\<down>"]) back
     apply (auto simp add:closure erasure typing)
   done
 
-  finally show ?thesis .
-qed
-
-lemma SkipREA_is_R2 : "`R2(II\<^bsub>rea\<^esub>)` = `II\<^bsub>rea\<^esub>`"
-proof-
-  have "`R2(II\<^bsub>rea\<^esub>)` = `(\<not>ok \<and> ($tr \<le> $tr\<acute>)) \<or> (ok' \<and> R2(II\<^bsub>REL_VAR - OKAY\<^esub>))`" 
-    apply (simp add: R2_def R1_def SkipREA_def R2s_def usubst typing defined closure)
-    apply(utp_pred_auto_tac)
-    done
-  thus ?thesis 
-    by (simp add:SkipRA_is_R2 SkipREA_def)
+  finally show ?thesis 
+    by(simp add:SkipR_as_SkipRA)
 qed
 
 subsection {* R3 Laws *}
@@ -849,7 +795,7 @@ subsection {* R3 Laws *}
 (* L1 R3-wait-true *)
 
 lemma R3_wait_true: 
-  "`(R3(P))\<^sub>t` = `(II\<^bsub>rea\<^esub>)\<^sub>t` "
+  "`(R3(P))\<^sub>t` = `II\<^sub>t` "
 by(simp add:R3_def usubst typing defined closure CondR_def)
 
 (* L2 R3-wait-false *)
@@ -857,16 +803,6 @@ by(simp add:R3_def usubst typing defined closure CondR_def)
 lemma R3_wait_false: 
   "`(R3(P))\<^sub>f` = `P\<^sub>f` "
 by(simp add:R3_def usubst typing defined closure CondR_def)
-
-(* L3 R3-okay' *)
-
-lemma R3_okay'_true: 
-  "(R3(P))\<^sup>t = `II\<^bsub>rea\<^esub>\<^sup>t \<lhd> $wait \<rhd>(P\<^sup>t)`"
-by(simp add:R3_def usubst typing defined closure)
-
-lemma R3_okay'_false: 
-  "(R3(P))\<^sup>f = `II\<^bsub>rea\<^esub>\<^sup>f \<lhd> $wait \<rhd>(P\<^sup>f)`"
-by(simp add:R3_def usubst typing defined closure)
 
 (* L4 closure-\<and>-R3 *)
 
@@ -903,20 +839,10 @@ by(metis is_healthy_def R3_CondR assms)
 
 (* L7 closure-sequence-R3 *)
 
-lemma R3_form : "`R3(P)` = `(\<not>ok \<and> $wait \<and> ($tr \<le> $tr\<acute>)) \<or> (ok \<and> $wait  \<and> II) \<or> (\<not>$wait \<and> P)`"
-  apply(simp add:R3_def SkipREA_CondR_SkipR CondR_def)
-  apply(utp_pred_auto_tac)
-done
+lemma R3_form : "`R3(P)` = `($wait  \<and> II) \<or> (\<not>$wait \<and> P)`"
+  by(simp add:R3_def CondR_def)
 
-lemma R3_form_2 : "`R3(P)` = `(\<not>ok \<and> $wait \<and> ($tr \<le> $tr\<acute>)) \<or> (ok \<and> $wait  \<and> II) \<or> (\<not>$wait \<and> P\<^sub>f )`"
-proof -
-  have "`\<not>$wait \<and> P` = `\<not>$wait \<and> P\<^sub>f`"
-    by (subst NotP_PVarPE_PSubstPE, simp_all add:typing)
-  thus ?thesis
-    by(simp add:R3_form)
-qed
-
-lemma R3_wait: "`R3(P) \<and> $wait` = `II\<^bsub>rea\<^esub> \<and> $wait`"
+lemma R3_wait: "`R3(P) \<and> $wait` = `II \<and> $wait`"
   apply (simp add:R3_def)
   apply (subst AndP_comm)
   apply (subst CondR_true_cond)
@@ -924,199 +850,61 @@ lemma R3_wait: "`R3(P) \<and> $wait` = `II\<^bsub>rea\<^esub> \<and> $wait`"
   apply (rule refl)
 done
 
-theorem R3_SemiR_closure [closure]:
+lemma wait_and_II: "`$wait \<and> II` =`$wait \<and> II \<and> $wait\<acute>`"
+  apply(simp add:SkipR_as_SkipRA)
+  apply(subst SkipRA_unfold[of "wait \<down>"])
+  apply(simp_all add:closure)
+  apply(subst SkipRA_unfold[of "wait \<down>"]) back
+  apply(simp_all add:closure)
+  apply(utp_pred_auto_tac)
+done
+
+theorem R3_SemiR_form:
   assumes
     "P \<in> WF_RELATION" "Q \<in> WF_RELATION"
-    "P is R3" "Q is R3" "Q is R1"
-  shows "(P ; Q) is R3"
-proof -
-  have "`(\<not>ok \<and> $wait \<and> ($tr \<le> $tr\<acute>));Q` = `\<not>ok \<and> $wait \<and> (($tr \<le> $tr\<acute>);Q)`"
-    apply(subst SemiR_AndP_left_precond)
-    apply (metis MkPlainP_UNDASHED PUNDASHED_WF_CONDITION R1_def R1_rel_closure WF_CONDITION_WF_RELATION)
-    apply (metis assms(2))
-    apply (metis TopD_cond_closure TopD_def)
-    apply(subst SemiR_AndP_left_precond)
-    apply (simp_all)
-    apply (metis R1_def R1_rel_closure TrueP_rel_closure utp_pred_simps(6))
-    apply (metis assms(2))
-    apply (metis MkPlainP_UNDASHED PUNDASHED_WF_CONDITION)
-    done
-  moreover have "`($tr \<le> $tr\<acute>) ; Q ` = `($tr \<le> $tr\<acute>)`"
-  proof-
-    have 1: "`(($tr \<le> $tr\<acute>) ; (\<not>ok \<and> $wait \<and> ($tr \<le> $tr\<acute>)))`=`($tr \<le> $tr\<acute>)`"
-      by (metis (hide_lams, no_types) Aida AndP_assoc)
-    have 2: "`(($tr \<le> $tr\<acute>);(ok \<and> $wait \<and> II))` is R1" 
-      apply(subst R1_SemiR_closure)
-      apply(simp_all)
-      apply (metis R1_def R1_rel_closure TrueP_rel_closure utp_pred_simps(6))
-      apply (metis AndP_rel_closure MkPlainP_UNDASHED PUNDASHED_WF_CONDITION SkipR_closure WF_CONDITION_WF_RELATION)
-      apply (metis R1_by_refinement order_refl)
-      apply (metis (full_types) AndP_comm Healthy_intro R1_SkipR R1_extend_AndP)
-      done
-    have 3: "`(($tr \<le> $tr\<acute>);(\<not>$wait \<and> Q))` is R1"
-      apply(subst R1_SemiR_closure)
-      apply(simp_all)
-      apply (metis R1_def R1_rel_closure TrueP_rel_closure utp_pred_simps(6))
-      apply (metis AndP_rel_closure MkPlainP_UNDASHED NotP_rel_closure PUNDASHED_WF_CONDITION WF_CONDITION_WF_RELATION assms(2))
-      apply (metis R1_by_refinement order_refl)  
-      apply (metis (full_types) AndP_comm R1_extend_AndP assms(5) is_healthy_def)
-      done
-    have "`($tr \<le> $tr\<acute>) ; Q` = `($tr \<le> $tr\<acute>) ; R3(Q)`"
-      by (metis Healthy_simp assms)
-    also have "... = `(($tr \<le> $tr\<acute>) ; (\<not>ok \<and> $wait \<and> ($tr \<le> $tr\<acute>))) \<or> (($tr \<le> $tr\<acute>);(ok \<and> $wait \<and> II)) \<or> (($tr \<le> $tr\<acute>);(\<not>$wait \<and> Q))`"
-      by(simp add:R3_form SemiR_OrP_distl)
-    also have "... = `($tr \<le> $tr\<acute>) \<or> R1(($tr \<le> $tr\<acute>);(ok \<and> $wait \<and> II)) \<or> R1(($tr \<le> $tr\<acute>);(\<not>$wait \<and> Q))`"
-      by(metis 1 2 3 is_healthy_def)
-    also have "... = `($tr \<le> $tr\<acute>)`"
-      by(utp_pred_auto_tac)
-    finally show ?thesis 
-      ..
-  qed
-  ultimately have 1: "`(\<not>ok \<and> $wait \<and> ($tr \<le> $tr\<acute>)) ; Q` = `\<not>ok \<and> $wait \<and> ($tr \<le> $tr\<acute>)`" by metis
-  have a : "`((($okay \<and> $wait \<and> II) \<and> ($okay)\<acute>) \<and> ($wait)\<acute>)` = `ok \<and> ok' \<and> $wait \<and> $wait\<acute> \<and> II`"
-    by (smt AndP_assoc AndP_comm ConvR_VarP_1 MkPlainP_UNDASHED PVAR_VAR_PUNDASHED_UNDASHED PVAR_VAR_pvdash)
-  have 2: "`(ok \<and> $wait \<and> II);Q` = `ok \<and> $wait \<and> II`"
-    proof -
-      have "`ok \<and> $wait \<and> II` = `ok \<and> $wait \<and> ($okay\<acute> = $okay) \<and> ($wait\<acute> = $wait) \<and> II`"
-        apply (simp add:SkipR_as_SkipRA)
-        apply (subst SkipRA_unfold[of "okay \<down>"])
-        apply(simp_all)
-        apply (metis MkPlainP_UNDASHED PVAR_VAR_PUNDASHED_UNDASHED)
-        apply(utp_pred_auto_tac)
-        apply (metis MkPlainP_UNDASHED PVAR_VAR_PUNDASHED_UNDASHED)
-        apply (subst SkipRA_unfold[of "okay \<down>"]) back
-        apply(simp_all)
-        apply (metis MkPlainP_UNDASHED PVAR_VAR_PUNDASHED_UNDASHED)
-        apply(utp_pred_auto_tac)
-        apply (metis MkPlainP_UNDASHED PVAR_VAR_PUNDASHED_UNDASHED)
-        apply (subst SkipRA_unfold[of "wait \<down>"])
-        apply(simp_all)
-        apply (metis MkPlainP_UNDASHED PVAR_VAR_PUNDASHED_UNDASHED)
-        apply(utp_pred_auto_tac)
-        apply (metis MkPlainP_UNDASHED PVAR_VAR_PUNDASHED_UNDASHED)
-        apply(utp_pred_auto_tac)
-        apply (subst SkipRA_unfold[of "wait \<down>"]) back
-        apply(simp_all)
-        apply (metis MkPlainP_UNDASHED PVAR_VAR_PUNDASHED_UNDASHED)
-        apply(utp_pred_auto_tac)
-        apply (metis MkPlainP_UNDASHED PVAR_VAR_PUNDASHED_UNDASHED)
-        apply(utp_pred_auto_tac)
-        apply(simp add:erasure typing defined closure)
-        apply (smt AndP_assoc AndP_idem)
-        done
-      also have "... = `ok \<and> ok' \<and> $wait \<and> $wait\<acute> \<and> II`"
-        by (smt AndP_assoc AndP_comm Aidb Aidc)
-      finally have "`(ok \<and> $wait \<and> II);R3(Q)` = `(ok \<and> ok' \<and> $wait \<and> $wait\<acute> \<and> II);R3(Q)`" 
-        by metis
-      also have "... = `(ok \<and> $wait \<and> II);(ok \<and> $wait \<and> R3(Q))`" 
-        apply(subst SemiR_AndP_right_precond)
-        apply (metis AndP_rel_closure MkPlainP_UNDASHED PUNDASHED_WF_CONDITION SkipR_closure WF_CONDITION_WF_RELATION)
-        apply (metis AndP_rel_closure MkPlainP_UNDASHED PUNDASHED_WF_CONDITION WF_CONDITION_WF_RELATION assms(2) assms(4) is_healthy_def)
-        apply (metis MkPlainP_UNDASHED PUNDASHED_WF_CONDITION)
-        apply(subst SemiR_AndP_right_precond)
-        apply (smt AndP_rel_closure ConvR_rel_closure MkPlainP_UNDASHED PUNDASHED_WF_CONDITION SkipR_closure WF_CONDITION_WF_RELATION)
-        apply (metis R3_rel_closure assms(2))
-        apply (metis MkPlainP_UNDASHED PUNDASHED_WF_CONDITION)
-        apply (metis a)
-        done
-      also have "... = `(ok \<and> $wait \<and> II);(ok \<and> $wait \<and> II)`"
-        proof -
-          have "`ok \<and> $wait \<and> R3(Q)` = `ok \<and> $wait \<and> II`" 
-            apply(simp add:R3_form) 
-            apply(utp_pred_auto_tac) 
-            done
-          thus ?thesis 
-            by metis
-        qed
-      also have "... = `(ok \<and> ok' \<and> $wait \<and> $wait\<acute> \<and> II);II`"
-        apply(subst SemiR_AndP_right_precond)
-        apply (metis AndP_rel_closure MkPlainP_UNDASHED PUNDASHED_WF_CONDITION SkipR_closure WF_CONDITION_WF_RELATION)
-        apply (metis (full_types) AndP_rel_closure MkPlainP_UNDASHED PUNDASHED_WF_CONDITION SkipR_closure WF_CONDITION_WF_RELATION)
-        apply (metis MkPlainP_UNDASHED PUNDASHED_WF_CONDITION)
-        apply(subst SemiR_AndP_right_precond)
-        apply (smt AndP_rel_closure ConvR_rel_closure MkPlainP_UNDASHED PUNDASHED_WF_CONDITION SkipR_closure WF_CONDITION_WF_RELATION)
-        apply (metis SkipR_closure)
-        apply (metis MkPlainP_UNDASHED PUNDASHED_WF_CONDITION)
-        apply (metis a)
-        done
-      also have "... = `ok \<and> ok' \<and> $wait \<and> $wait\<acute> \<and> II`"by (metis SemiR_SkipR_right)
-      also have "... = `ok \<and> $wait \<and> II`"
-      proof -
-        have "`ok \<and> ok' \<and> $wait \<and> $wait\<acute> \<and> II` =  `ok \<and> $wait \<and> ($okay\<acute> = $okay) \<and> ($wait\<acute> = $wait) \<and> II`"
-          by (smt AndP_assoc AndP_comm Aidb Aidc)
-        also have "... = `ok \<and> $wait \<and> II`"
-          apply (simp add:SkipR_as_SkipRA)
-          apply (subst SkipRA_unfold[of "okay \<down>"])
-          apply(simp_all)
-          apply (metis MkPlainP_UNDASHED PVAR_VAR_PUNDASHED_UNDASHED)
-          apply(utp_pred_auto_tac)
-          apply (metis MkPlainP_UNDASHED PVAR_VAR_PUNDASHED_UNDASHED)
-          apply (subst SkipRA_unfold[of "okay \<down>"]) back
-          apply(simp_all)
-          apply (metis MkPlainP_UNDASHED PVAR_VAR_PUNDASHED_UNDASHED)
-          apply(utp_pred_auto_tac)
-          apply (metis MkPlainP_UNDASHED PVAR_VAR_PUNDASHED_UNDASHED)
-          apply (subst SkipRA_unfold[of "wait \<down>"])
-          apply(simp_all)
-          apply (metis MkPlainP_UNDASHED PVAR_VAR_PUNDASHED_UNDASHED)
-          apply(utp_pred_auto_tac)
-          apply (metis MkPlainP_UNDASHED PVAR_VAR_PUNDASHED_UNDASHED)
-          apply(utp_pred_auto_tac)
-          apply (subst SkipRA_unfold[of "wait \<down>"]) back
-          apply(simp_all)
-          apply (metis MkPlainP_UNDASHED PVAR_VAR_PUNDASHED_UNDASHED)
-          apply(utp_pred_auto_tac)
-          apply (metis MkPlainP_UNDASHED PVAR_VAR_PUNDASHED_UNDASHED)
-          apply(utp_pred_auto_tac)
-          apply(simp add:erasure typing defined closure)
-          apply (smt AndP_assoc AndP_idem)
-          done
-        finally show ?thesis
-          ..
-      qed
-      finally show ?thesis 
-        by (metis assms(4) is_healthy_def)
-    qed
-  have 3: "`(\<not> $wait \<and> P);Q` = `\<not> $wait \<and> (P;Q)`"
-    by(subst SemiR_AndP_left_precond, simp_all add:assms, utp_pred_auto_tac)
-  have "`P ; Q` = `R3(P) ; Q`" 
-    by (metis assms(3) is_healthy_def)
-  also have "... = `(\<not>ok \<and> $wait \<and> ($tr \<le> $tr\<acute>));Q  \<or> (ok \<and> $wait \<and> II);Q \<or> (\<not> $wait \<and> P);Q`" 
-    by(simp add:R3_form SemiR_OrP_distr)
-  also have "... = `(\<not>ok \<and> $wait \<and> ($tr \<le> $tr\<acute>))  \<or> (ok \<and> $wait \<and> II) \<or> (\<not> $wait \<and> (P;Q))`"
-    by (metis "1" "2" "3") 
-  finally show ?thesis 
-    by (simp add:R3_form is_healthy_def)
-qed
+  shows "R3(P);R3(Q) = R3(P;R3(Q))"
+    apply(simp add:R3_form SemiR_OrP_distl SemiR_OrP_distr)
+    apply(subst SemiR_AndP_right_precond)
+    apply(simp_all add:closure typing defined WF_RELATION_UNREST unrest urename)
+    apply(subst SemiR_AndP_right_precond)
+    apply(simp_all add:closure typing defined WF_RELATION_UNREST unrest urename assms(1))
+    apply(subst SemiR_AndP_right_precond)
+    apply(simp_all add:closure typing defined WF_RELATION_UNREST unrest urename assms(2))
+    apply(subst SemiR_AndP_right_precond)
+    apply(simp_all add:closure typing defined WF_RELATION_UNREST unrest urename assms(1) assms(2))
+    apply(subst SemiR_AndP_right_precond)
+    apply(simp_all add:closure typing defined WF_RELATION_UNREST unrest urename assms(1) assms(2))
+    apply(subst SemiR_AndP_right_precond)
+    apply(simp_all add:closure typing defined WF_RELATION_UNREST unrest urename assms(1) assms(2))
+    apply(subst wait_and_II) back
+    apply(subst wait_and_II) back
+    apply(simp add:AndP_OrP_distl AndP_assoc[THEN sym])
+    apply(subst SemiR_AndP_left_precond[where c="`\<not>$wait`"])
+    apply(simp_all add:closure typing defined WF_RELATION_UNREST unrest urename assms(1) assms(2))
+    apply(simp add:AndP_contra)
+    apply(utp_pred_auto_tac)
+done
+
+lemma R3_SemiR_closure[closure]: 
+  assumes "P \<in> WF_RELATION" "Q \<in> WF_RELATION" "P is R3" "Q is R3"
+  shows "P ; Q is R3"
+by (metis Healthy_intro Healthy_simp R3_SemiR_form assms(1) assms(2) assms(3) assms(4))
 
 (* L8 R3-idempotent *)
 
 lemma R3_idempotent: "`R3(R3(P))` = `R3(P)`" 
   by (utp_pred_auto_tac)
 
-(* L9 commutativity-R3-H2 *)
-
-lemma H2_R3_commute: 
-  assumes "P \<in> WF_RELATION"
-  shows "H2 (R3 P) = R3 (H2 P)" 
-  apply(simp add:R3_def CondR_def H2_def SemiR_OrP_distr)
-  apply(subst SemiR_AndP_left_precond[of _ _ "`$wait`"])
-  apply(simp_all add:SkipREA_rel_closure J_closure MkPlainP_UNDASHED PUNDASHED_WF_CONDITION)
-  apply(subst SemiR_AndP_left_precond[of _ _ "`\<not>$wait`"])
-  apply(simp_all add:assms J_closure MkPlainP_UNDASHED NotP_cond_closure PUNDASHED_WF_CONDITION) 
-  apply (metis H2_SkipREA H2_def)
-  done
-
 (* L10 commutativity-R3-R1 *)
 
 lemma R1_R3_commute: "R1 (R3 P) = R3 (R1 P)" 
 proof - 
-  have "R1 (R3 P) = `(II\<^bsub>rea\<^esub> \<lhd> $wait \<rhd> P) \<and> ($tr \<le> $tr\<acute>)`" 
+  have "R1 (R3 P) = `(II \<lhd> $wait \<rhd> P) \<and> ($tr \<le> $tr\<acute>)`" 
     by utp_rel_tac
-  also have "... = `(II\<^bsub>rea\<^esub> \<and> ($tr \<le> $tr\<acute>)) \<lhd> $wait \<rhd> (P \<and> ($tr \<le> $tr\<acute>))`" 
+  also have "... = `(II \<and> ($tr \<le> $tr\<acute>)) \<lhd> $wait \<rhd> (P \<and> ($tr \<le> $tr\<acute>))`" 
     by utp_pred_auto_tac
-  also have "... = `II\<^bsub>rea\<^esub> \<lhd> $wait \<rhd> (P \<and> ($tr \<le> $tr\<acute>))`" 
-    by (metis R1_def SkipREA_is_R1)
+  also have "... = `II \<lhd> $wait \<rhd> (P \<and> ($tr \<le> $tr\<acute>))`" 
+    by (metis R1_SkipR R1_def)
   ultimately show ?thesis by utp_pred_auto_tac
 qed
 
@@ -1125,46 +913,26 @@ qed
 theorem R2_R3_commute: 
   "R2 (R3 P) = R3 (R2 P)" 
 proof - 
-  have "R2 (R3 P) = `R2(II\<^bsub>rea\<^esub>) \<lhd> R2s($wait) \<rhd> R2(P)`" 
+  have "R2 (R3 P) = `R2(II) \<lhd> R2s($wait) \<rhd> R2(P)`" 
     by (simp add:R3_def R2_CondR)
-  also have "... = `II\<^bsub>rea\<^esub> \<lhd> $wait \<rhd> R2(P)`"
-    by (simp add: SkipREA_is_R2 R2s_def usubst typing defined closure)
+  also have "... = `II \<lhd> $wait \<rhd> R2(P)`"
+    apply(simp add:R2s_def usubst typing defined closure)
+    by (metis SkipRA_is_R2)
   finally show ?thesis 
     by (simp add: R3_def R2_def)
 qed
 
-(* L12 R3-H1-sub-commutativity *)
-
-lemma R3_H1_sub_commute: 
-  "H1 (R3 P) = H1 (R3 (H1 P))"
-by(utp_pred_auto_tac)
-
-(* L13 R3-H1-R1-sub-commutativity *)
-
-lemma R3_H1_R1_sub_commute: 
-  "R3 (R1 (H1 P)) = R1 (H1 (R3 P))"
-proof -
-  have "R3 (R1 (H1 P)) = `($wait \<and> II\<^bsub>rea\<^esub>) \<or> (\<not>$wait \<and> ($tr\<le>$tr\<acute>) \<and> \<not>ok) \<or> (\<not>$wait \<and> ($tr\<le>$tr\<acute>) \<and> P)`" 
-    by utp_pred_auto_tac
-  also have "... = `($wait \<and> II\<^bsub>rea\<^esub> \<and> ($tr\<le>$tr\<acute>)) \<or> (\<not>$wait \<and> ($tr\<le>$tr\<acute>) \<and> \<not>ok) \<or> (\<not>$wait \<and> ($tr\<le>$tr\<acute>) \<and> P)`"
-    proof -
-      have "`II\<^bsub>rea\<^esub>` = `II\<^bsub>rea\<^esub> \<and> ($tr\<le>$tr\<acute>)` "
-        by (metis R1_def SkipREA_is_R1)
-      thus ?thesis 
-        by metis
-    qed
-  finally show ?thesis 
-    by utp_pred_auto_tac
-qed
-
 (* Additional Lemmas *)
 
-lemma R3_SkipREA: "`R3(II\<^bsub>rea\<^esub>)` = `II\<^bsub>rea\<^esub>`"
+lemma R3_SkipREA: "`R3(II)` = `II`"
   by (simp add:R3_def CondR_idem)
 
-lemma R3_monotonic: "P \<sqsubseteq> Q \<Longrightarrow> R3(P) \<sqsubseteq> R3(Q)" 
-  by utp_pred_tac
+declare CondR_def [evalp]
+declare less_eq_WF_PREDICATE_def [evalp]
 
+lemma R3_monotonic: "P \<sqsubseteq> Q \<Longrightarrow> R3(P) \<sqsubseteq> R3(Q)"
+  by utp_poly_tac 
+  
 subsection {* RH Laws *}
 
 lemma RH_is_R1:
@@ -1186,55 +954,60 @@ lemma R_intro: "\<lbrakk> P is R1; P is R2; P is R3 \<rbrakk> \<Longrightarrow> 
 
 lemma R1_true_left_zero: 
   assumes "P is R1" "P is R3" "P \<in> WF_RELATION"
-  shows "`($tr \<le> $tr\<acute>) ; P` = `($tr \<le> $tr\<acute>)`"
+  shows "`($tr \<le> $tr\<acute>) ; P` = `($tr \<le> $tr\<acute>) \<and> ($wait\<acute> \<or> ($tr \<le> $tr\<acute>);P\<^sub>f)`"
 proof -
-  have 1: "`(($tr \<le> $tr\<acute>) ; (\<not>ok \<and> $wait \<and> ($tr \<le> $tr\<acute>)))`=`($tr \<le> $tr\<acute>)`"
-    by (metis (hide_lams, no_types) Aida AndP_assoc)
-  have 2: "`(($tr \<le> $tr\<acute>);(ok \<and> $wait \<and> II))` is R1" 
-    apply(subst R1_SemiR_closure)
-    apply(simp_all)
-    apply (metis R1_def R1_rel_closure TrueP_rel_closure utp_pred_simps(6))
-    apply (metis AndP_rel_closure MkPlainP_UNDASHED PUNDASHED_WF_CONDITION SkipR_closure WF_CONDITION_WF_RELATION)
-    apply (metis R1_by_refinement order_refl)
-    apply (metis (full_types) AndP_comm Healthy_intro R1_SkipR R1_extend_AndP)
-    done
-  have 3: "`(($tr \<le> $tr\<acute>);(\<not>$wait \<and> P))` is R1"
-    apply(subst R1_SemiR_closure)
-    apply(simp_all)
-    apply (metis R1_def R1_rel_closure TrueP_rel_closure utp_pred_simps(6))
-    apply (metis AndP_rel_closure MkPlainP_UNDASHED NotP_rel_closure PUNDASHED_WF_CONDITION WF_CONDITION_WF_RELATION assms(3))
-    apply (metis R1_by_refinement order_refl)  
-    apply (metis (full_types) AndP_comm R1_extend_AndP RH_is_R1 assms(1) is_healthy_def)
-    done
-  have "`($tr \<le> $tr\<acute>) ; P` = `($tr \<le> $tr\<acute>) ; R3(P)`"
-    by (metis Healthy_simp RH_is_R3 assms)
-  also have "... = `(($tr \<le> $tr\<acute>) ; (\<not>ok \<and> $wait \<and> ($tr \<le> $tr\<acute>))) \<or> (($tr \<le> $tr\<acute>);(ok \<and> $wait \<and> II)) \<or> (($tr \<le> $tr\<acute>);(\<not>$wait \<and> P))`"
-    by(simp add:R3_form SemiR_OrP_distl)
-  also have "... = `($tr \<le> $tr\<acute>) \<or> R1(($tr \<le> $tr\<acute>);(ok \<and> $wait \<and> II)) \<or> R1(($tr \<le> $tr\<acute>);(\<not>$wait \<and> P))`"
-    by(metis 1 2 3 is_healthy_def)
-  also have "... = `($tr \<le> $tr\<acute>)`"
-    by(utp_pred_auto_tac)
-  finally show ?thesis 
-    ..
+have 1: "`($wait\<acute> \<and> II)` = `($wait \<and> $wait\<acute> \<and> II)`"
+  apply(simp add:SkipR_as_SkipRA)
+  apply(subst SkipRA_unfold[of "wait \<down>"])
+  apply(simp_all add:closure)
+  apply(subst SkipRA_unfold[of "wait \<down>"])back
+  apply(simp_all add:closure)
+  apply(utp_pred_auto_tac)
+  done
+have "P = `($wait \<and> II) \<or> (\<not>$wait \<and> P)`"
+  by (metis Healthy_simp R3_form assms(2))
+hence "`($tr \<le> $tr\<acute>) ; P` = `($tr \<le> $tr\<acute>) ; ($wait \<and> II) \<or> ($tr \<le> $tr\<acute>) ; (\<not>$wait \<and> P)`"
+  by (metis (hide_lams, no_types) SemiR_OrP_distl)
+also have "... = `($tr \<le> $tr\<acute>) ; ($wait \<and> $wait\<acute> \<and> II ) \<or> ($tr \<le> $tr\<acute>) ; (\<not>$wait \<and> P)`"
+  by (metis AndP_comm wait_and_II)
+also have "... = `($tr \<le> $tr\<acute>) ; (II \<and> $wait\<acute>) \<or> ($tr \<le> $tr\<acute>) ; (\<not>$wait \<and> P)`"
+  by (metis "1" AndP_comm)
+also have "... = `(($tr \<le> $tr\<acute>) \<and> $wait\<acute>) \<or> ($tr \<le> $tr\<acute>) ; (\<not>$wait \<and> P\<^sub>f)`"
+  apply(subst SemiR_AndP_right_postcond)
+  apply(simp_all add:closure)
+  apply (smt R1_def R1_rel_closure TrueP_rel_closure utp_pred_simps(6))
+  apply(subst NotP_PVarPE_PSubstPE)
+  apply(simp_all add:closure typing)
+  done
+also have "... =  `(($tr \<le> $tr\<acute>) \<and> $wait\<acute>) \<or> ($tr \<le> $tr\<acute>) ; P\<^sub>f`"
+  apply(subst SemiR_remove_middle_unrest1[of _ _ "{wait \<down>}"])
+  apply(simp_all add:closure typing defined erasure unrest)
+  apply (smt R1_def R1_rel_closure TrueP_rel_closure utp_pred_simps(6))
+  apply(subst SubstP_rel_closure)
+  apply(simp_all add:assms closure typing defined WF_RELATION_UNREST unrest)
+  done
+also have "... = `(($tr \<le> $tr\<acute>) \<and> $wait\<acute>) \<or> R1(($tr \<le> $tr\<acute>) ; P\<^sub>f)`"
+  proof-
+    have "`P\<^sub>f` is R1"
+      apply(simp add:is_healthy_def R1_wait_false[THEN sym])
+      by (metis Healthy_simp assms(1))
+    hence "`($tr \<le> $tr\<acute>) ; P\<^sub>f` is R1"
+      apply(subst R1_SemiR_closure)
+      apply(simp_all add:closure is_healthy_def R1_def assms typing defined WF_RELATION_UNREST unrest)
+      done
+    thus ?thesis 
+      by (metis is_healthy_def)
+    qed
+finally show ?thesis 
+  by(utp_pred_auto_tac) 
 qed
 
 (* L2 restricted-identity *)
 
-lemma SkipREA_restricted_identity:
+lemma Skip_identity:
   assumes "P is RH" "P \<in> WF_RELATION"
-  shows " `II\<^bsub>rea\<^esub>; P` = `P \<lhd> ok \<rhd> ($tr \<le> $tr\<acute>)`"
-  apply (simp add:SkipREA_CondR_SkipR CondR_def SemiR_OrP_distr)
-  apply (subst SemiR_AndP_left_precond[of _ _ "`ok`"])
-  apply (simp_all add:SkipR_closure assms(2) MkPlainP_UNDASHED PUNDASHED_WF_CONDITION)
-  apply (subst SemiR_AndP_left_precond[of _ _ "`\<not>ok`"])
-  apply (simp_all add:assms(2))
-  apply (metis R1_def R1_rel_closure TrueP_rel_closure utp_pred_simps(6))
-  apply (metis TopD_cond_closure TopD_def)
-  apply (subst R1_true_left_zero)
-  apply (simp_all add:assms)
-  apply (metis RH_is_R1 assms(1))
-  apply (metis RH_is_R3 assms(1))
-  done
+  shows " `II ; P` = P"
+by (metis SemiR_SkipR_left)
 
 (* L3 R-wait-false *)
 
@@ -1245,68 +1018,8 @@ by(simp add:RH_def R1_wait_false R2_wait_false R3_wait_false)
 (* L4 R-wait-true *)
 
 lemma RH_wait_true: 
-  "`(RH(P))\<^sub>t` = `II\<^bsub>rea\<^esub>\<^sub>t`"
-proof -
-  have 1: "`II\<^bsub>rea\<^esub>\<^sub>t` = `(\<not>ok \<and> ($tr \<le> $tr\<acute>)) \<or> (ok' \<and> $wait\<acute> \<and> II\<^bsub>REL_VAR - {okay\<down>, okay\<down>\<acute>} - {wait\<down>, wait\<down>\<acute>}\<^esub>)`"
-    apply(simp add:SkipREA_def usubst typing defined closure)
-    apply (metis (hide_lams, no_types) Aidd PVAR_VAR_pvdash)
-    done
-  have "`(RH(P))\<^sub>t` = R1 (R2 `II\<^bsub>rea\<^esub>\<^sub>t`)"
-    by(simp add: RH_def R1_wait_true R2_wait_true R3_wait_true)
-  also from 1 have "... = R1 (R2 `(\<not>ok \<and> ($tr \<le> $tr\<acute>)) \<or> (ok' \<and> $wait\<acute> \<and> II\<^bsub>REL_VAR - {okay\<down>, okay\<down>\<acute>} - {wait\<down>, wait\<down>\<acute>}\<^esub>)`)"
-    by(metis)
-  also have "... = `R1 (\<not>ok) \<or> R1 (ok' \<and> $wait\<acute> \<and> (($tr\<acute> - $tr) = \<langle>\<rangle>) \<and> II\<^bsub>REL_VAR - {okay\<down>, okay\<down>\<acute>} - {wait\<down>, wait\<down>\<acute>} - {tr\<down>, tr\<down>\<acute>}\<^esub>)`" 
-    apply(simp add: R2_def R1_idempotent)
-    apply(subst SkipRA_unfold[of "tr \<down>"])
-    apply(simp_all)
-    apply (metis MkPlain_UNDASHED PVAR_VAR_MkPVAR)
-    apply (metis MkPlain_UNDASHED PVAR_VAR_MkPVAR UNDASHED_dash_DASHED)
-    apply (metis MkPlain_UNDASHED PVAR_VAR_MkPVAR)
-    apply (smt HOMOGENEOUS_REL_VAR HOMOGENEOUS_empty HOMOGENEOUS_insert HOMOGENEOUS_minus MkPlainP_UNDASHED PVAR_VAR_PUNDASHED_UNDASHED)
-    apply(simp add:R2s_def usubst typing defined closure R1_OrP)
-    done
-  also have "... = `(\<not>ok \<and> ($tr \<le> $tr\<acute>)) \<or> (ok' \<and> $wait\<acute> \<and> R1(($tr\<acute> - $tr) = \<langle>\<rangle>) \<and> II\<^bsub>REL_VAR - {okay\<down>, okay\<down>\<acute>} - {wait\<down>, wait\<down>\<acute>} - {tr\<down>, tr\<down>\<acute>}\<^esub>)`"
-    by(utp_pred_auto_tac)
-  also have "... = `(\<not>ok \<and> ($tr \<le> $tr\<acute>)) \<or> (ok' \<and> $wait\<acute> \<and> ($tr\<acute> = $tr) \<and> II\<^bsub>REL_VAR - {okay\<down>, okay\<down>\<acute>} - {wait\<down>, wait\<down>\<acute>} - {tr\<down>, tr\<down>\<acute>}\<^esub>)`"
-    by (smt R1_def tr_prefix_as_nil)
-  also have "... = `(\<not>ok \<and> ($tr \<le> $tr\<acute>)) \<or> (ok' \<and> $wait\<acute> \<and> II\<^bsub>REL_VAR - {okay\<down>, okay\<down>\<acute>} - {wait\<down>, wait\<down>\<acute>}\<^esub>)`"
-    apply(subst SkipRA_unfold[of "tr \<down>"]) back
-    apply(simp_all)
-    apply (metis MkPlain_UNDASHED PVAR_VAR_MkPVAR)
-    apply (metis MkPlain_UNDASHED PVAR_VAR_MkPVAR UNDASHED_dash_DASHED)
-    apply (metis MkPlain_UNDASHED PVAR_VAR_MkPVAR)
-    apply (smt HOMOGENEOUS_REL_VAR HOMOGENEOUS_empty HOMOGENEOUS_insert HOMOGENEOUS_minus MkPlainP_UNDASHED PVAR_VAR_PUNDASHED_UNDASHED)
-    apply(simp add:erasure typing closure defined)
-    done
-  also from 1 have "... = `II\<^bsub>rea\<^esub>\<^sub>t`" 
-    by metis
-  finally show ?thesis
-    ..
-qed
-
-(* L5 R-okay' *)
-
-lemma RH_okay'_true: 
-  "(RH(P))\<^sup>t = `II\<^bsub>rea\<^esub>\<^sup>t \<lhd> $wait \<rhd>R1(R2(P\<^sup>t))`"
-proof-
-  have "(R1(R2(P)))\<^sup>t = R1(R2(P\<^sup>t))" 
-    by (metis R1_okay'_true R2_okay'_true)
-  hence "(R3(R1(R2(P))))\<^sup>t = `II\<^bsub>rea\<^esub>\<^sup>t \<lhd> $wait \<rhd>R1(R2(P\<^sup>t))`" 
-    by (smt R3_okay'_true)
-  thus ?thesis 
-    by(simp add:RH_def R2_R3_commute R1_R3_commute)
-qed
-
-lemma RH_okay'_false: 
-  "(RH(P))\<^sup>f = `II\<^bsub>rea\<^esub>\<^sup>f \<lhd> $wait \<rhd>R1(R2(P\<^sup>f))`"
-proof-
-  have "(R1(R2(P)))\<^sup>f = R1(R2(P\<^sup>f))" 
-    by (metis R1_okay'_false R2_okay'_false)
-  hence "(R3(R1(R2(P))))\<^sup>f = `II\<^bsub>rea\<^esub>\<^sup>f \<lhd> $wait \<rhd>R1(R2(P\<^sup>f))`" 
-    by (smt R3_okay'_false)
-  thus ?thesis 
-    by(simp add:RH_def R2_R3_commute R1_R3_commute)
-qed
+  "`(RH(P))\<^sub>t` = `II\<^sub>t`"
+by(simp add:RH_def R2_R3_commute R1_R3_commute R3_wait_true)
 
 (* L6 closure-\<and>-R *)
 
@@ -1353,42 +1066,11 @@ proof -
 qed
 
 (* L9 closure-sequence-R *)
-(*
+
 lemma RH_SemiR_closure:
   assumes "P \<in> WF_RELATION" "Q\<in> WF_RELATION" "P is RH" "Q is RH"
   shows "`P ; Q` is RH"
-proof -
-  have "`R3(P ; Q)` = `P ; Q`"
-    by (metis Healthy_simp R3_SemiR_closure RH_is_R1 RH_is_R3 assms(1) assms(2) assms(3) assms(4))
-  hence "`R2(R3(P ; Q))` = `P ; Q`" 
-    by (metis R2_SemiR_closure RH_is_R2 assms is_healthy_def)
-  hence "`R1(R2(R3(P ; Q)))` = `P ; Q`" 
-    by (metis R1_idempotent R2_def)
-  thus ?thesis by(simp add:is_healthy_def RH_def)
-qed
-*)
-lemma RH_expansion:
-  "RH(P \<turnstile> Q) = `(\<not>ok \<and> ($tr \<le> $tr\<acute>)) \<or> (ok \<and> $wait \<and> II) \<or> (ok \<and> \<not>$wait \<and> R2(\<not>P)) \<or> (ok \<and> \<not>$wait \<and> ok' \<and> R2(Q))`"
-apply(simp add:RH_def DesignD_def R2_R3_commute)
-apply(simp add: R2_def R2s_def usubst typing defined closure R1_R3_commute R1_idempotent)
-apply(simp add:R3_form R1_def)
-apply(utp_pred_auto_tac)
-done
-
-lemma RH_form: 
-  assumes "P \<in> WF_RELATION" "P is RH"
-  shows "P = `(\<not>ok \<and> $wait \<and> ($tr \<le> $tr\<acute>)) \<or> (ok \<and> $wait \<and> II) \<or> (\<not>$wait \<and> R2(P\<^sub>f))`"
-proof-
-  have "P = RH P" by(metis is_healthy_def assms(2))
-  thus ?thesis
-  apply(simp add:RH_def R2_R3_commute R1_R3_commute)
-  apply(simp add:R3_form_2 R1_def)
-  apply(simp add:usubst typing defined closure)
-  apply(simp add:R2_wait_false)
-  apply(simp add:R2_def R1_def)
-  apply (metis (hide_lams, no_types) R1_def R1_idempotent)
-  done
-qed
+by (metis R1_SemiR_closure R2_SemiR_closure R3_SemiR_closure RH_is_R1 RH_is_R2 RH_is_R3 R_intro assms(1) assms(2) assms(3) assms(4))
 
 subsection {* The theory of Reactive Processes *}
 
