theories/theories/utp_acp_old.thy
@@ -1,0 +1,511 @@
+(******************************************************************************)
+(* Project: Mechanisation of the UTP                                          *)
+(* File: utp_acp.thy                                                          *)
+(* Authors: Samuel Canham and Simon Foster, University of York                *)
+(******************************************************************************)
+
+header {* ACP Processes *}
+
+theory utp_acp
+imports 
+  utp_designs
+  utp_theory
+  utp_reactive
+begin
+
+definition ACP1 :: "'a WF_PREDICATE \<Rightarrow> 'a WF_PREDICATE" where
+"ACP1 P = `P \<and> (ok \<and> ($tr\<acute> = $tr) \<Rightarrow> $wait\<acute>)` "
+
+definition \<delta> :: "'a WF_PREDICATE" where
+"\<delta> = `R3($tr\<acute> =$tr \<and> $wait\<acute>)`"
+
+definition B :: "'a WF_PREDICATE" where
+"B = `($tr\<acute> = $tr \<and> $wait\<acute>) \<or> ($tr < $tr\<acute>)`"
+
+definition \<Phi> :: "'a WF_PREDICATE \<Rightarrow> 'a WF_PREDICATE" where
+"\<Phi>(P) = `RH(B \<and> P)`"
+
+definition doA :: "('m EVENT, 'm) WF_PEXPRESSION \<Rightarrow> 'm WF_PREDICATE" where
+"doA(a) = `\<Phi>(a \<notin> $ref\<acute> \<lhd> $wait\<acute> \<rhd> ($tr^\<langle>a\<rangle> =$tr\<acute>))`"
+
+definition alternative :: "'a WF_PREDICATE \<Rightarrow> 'a WF_PREDICATE \<Rightarrow> 'a WF_PREDICATE" ("_ +\<^bsub>ACP\<^esub> _") where
+"(P +\<^bsub>ACP\<^esub> Q) = `(P \<and> Q) \<lhd> \<delta> \<rhd> (P \<or> Q)`"
+
+declare ACP1_def [eval,evalr,evalrx]
+declare \<delta>_def [eval,evalr,evalrx]
+declare B_def [eval,evalr,evalrx]
+declare \<Phi>_def [eval,evalr,evalrx]
+declare doA_def [eval,evalr,evalrx]
+declare alternative_def [eval,evalr,evalrx]
+
+syntax 
+  "_upred_doA" :: "uexpr \<Rightarrow> upred" ("do\<A>'(_')")
+  "_upred_alternative" :: "upred \<Rightarrow> upred \<Rightarrow> upred" ("_ + _")
+
+translations
+  "_upred_doA a" == "CONST doA a"
+  "_upred_alternative P Q" == "CONST alternative P Q"
+
+declare \<delta>_def [eval, evalr, evalrr, evalrx]
+declare doA_def [eval, evalr, evalrr, evalrx]
+declare \<Phi>_def [eval, evalr, evalrr, evalrx]
+declare B_def [eval, evalr, evalrr, evalrx]
+
+subsection {* Closure Laws *}
+
+lemma ACP1_rel_closure [closure]:
+  "P \<in> WF_RELATION \<Longrightarrow> ACP1(P) \<in> WF_RELATION"
+  by(simp add:ACP1_def closure typing defined unrest)
+
+lemma \<delta>_rel_closure [closure]:
+  "`\<delta>` \<in> WF_RELATION"
+  apply(simp add:\<delta>_def)
+  apply(subst R3_rel_closure)
+  apply(simp_all add:closure typing defined unrest)
+  done
+
+lemma B_rel_closure [closure]:
+  "`B` \<in> WF_RELATION"
+  by (simp add:B_def closure typing defined unrest WF_RELATION_UNREST)
+
+lemma \<Phi>_rel_closure [closure]:
+  "P \<in> WF_RELATION \<Longrightarrow> `\<Phi>(P)` \<in> WF_RELATION"
+  by(simp add:\<Phi>_def closure)
+
+lemma doA_rel_closure [closure]:
+  "NON_REL_VAR \<sharp> a \<Longrightarrow> `doA(a)` \<in> WF_RELATION"
+  by (simp add:doA_def closure typing defined unrest WF_RELATION_UNREST)
+  
+lemma Alternative_rel_closure [closure]:
+  "P \<in> WF_RELATION \<Longrightarrow> Q \<in> WF_RELATION \<Longrightarrow> (P +\<^bsub>ACP\<^esub> Q) \<in> WF_RELATION"
+  by(simp add:alternative_def closure)
+
+subsection {* ACP1 Laws *}
+
+lemma ACP1_idempotent: "ACP1(ACP1(P)) = ACP1(P)" 
+  by (simp add:ACP1_def, utp_pred_tac)
+
+lemma ACP1_monotonic: 
+  "P \<sqsubseteq> Q \<Longrightarrow> ACP1(P) \<sqsubseteq> ACP1(Q)" 
+  by (simp add:ACP1_def, utp_pred_auto_tac)
+
+lemma ACP1_R1_commute: 
+  "ACP1(R1(P)) = R1(ACP1(P))" 
+  by (simp add:ACP1_def, utp_pred_auto_tac)
+
+lemma ACP1_R2_commute: "ACP1(R2(P)) = R2(ACP1(P))" 
+proof -
+  have "R2(ACP1(P)) = `R2(P) \<and> (ok \<and> \<langle>\<rangle> = ($tr\<acute> - $tr) \<Rightarrow> $wait\<acute>)`"
+    by (simp add:ACP1_def R2_def R2s_def usubst typing defined closure, utp_pred_auto_tac)
+
+  also have "... = `R2(P) \<and> ($tr \<le> $tr\<acute>) \<and> (ok \<and> \<langle>\<rangle> = ($tr\<acute> - $tr) \<Rightarrow> $wait\<acute>)`"
+    by (smt AndP_assoc AndP_idem R1_def R2_def)
+
+  also have "... = `R2(P) \<and> ($tr \<le> $tr\<acute>) \<and> (($tr \<le> $tr\<acute>) \<and> ok \<and> \<langle>\<rangle> = ($tr\<acute> - $tr) \<Rightarrow> $wait\<acute>)`"
+    by (metis (hide_lams, no_types) ImpliesP_AndP_pre)
+
+  also have "... = `R2(P) \<and> (($tr \<le> $tr\<acute>) \<and> ok \<and> \<langle>\<rangle> = ($tr\<acute> - $tr) \<Rightarrow> $wait\<acute>)`"
+    by (smt AndP_assoc AndP_idem R1_def R2_def)
+
+  also have "... = `R2(P) \<and> (ok \<and> \<langle>\<rangle> = ($tr\<acute> - $tr) \<and> ($tr \<le> $tr\<acute>) \<Rightarrow> $wait\<acute>)`"
+    by (smt AndP_assoc AndP_comm)
+
+  also have "... = `R2(P) \<and> (ok \<and> ($tr\<acute> = $tr) \<Rightarrow> $wait\<acute>)`"
+    by (metis (hide_lams, no_types) EqualP_sym tr_prefix_as_nil)
+
+  finally show ?thesis 
+    by (simp add:ACP1_def) 
+qed
+
+lemma ACP1_R3_commute: "ACP1 (R3 P) = R3 (ACP1 P)" 
+proof -
+  have "ACP1 (R3 P) = `($wait \<and> \<not> ok \<and> ($tr \<le> $tr\<acute>)) \<or> (ok' \<and> $wait \<and> II\<^bsub>REL_VAR - {okay\<down>, okay\<down>\<acute>}\<^esub> \<and> ( ok \<and> ($tr\<acute> =$tr) \<Rightarrow> $wait\<acute>)) \<or> (\<not>$wait \<and> P \<and> (ok \<and> ($tr\<acute> =$tr) \<Rightarrow> $wait\<acute>))`" 
+    by (simp add:ACP1_def R3_def SkipREA_def CondR_def, utp_pred_auto_tac)
+
+  also have "... = `($wait \<and> \<not> ok \<and> ($tr \<le> $tr\<acute>)) \<or> (ok' \<and> $wait \<and> $wait\<acute> \<and> II\<^bsub>REL_VAR - {okay\<down>, okay\<down>\<acute>}\<^esub> \<and> ( ok \<and> ($tr\<acute> =$tr) \<Rightarrow> $wait\<acute>)) \<or> (\<not>$wait \<and> P \<and> ( ok \<and> ($tr\<acute> =$tr) \<Rightarrow> $wait\<acute>))`" 
+    sorry
+
+  also have "... = `($wait \<and> \<not> ok \<and> ($tr \<le> $tr\<acute>)) \<or> (ok' \<and> $wait \<and> $wait\<acute> \<and> II\<^bsub>REL_VAR - {okay\<down>, okay\<down>\<acute>}\<^esub>) \<or> (\<not>$wait \<and> P \<and> ( ok \<and> ($tr\<acute> =$tr) \<Rightarrow> $wait\<acute>))`" 
+    by (utp_pred_auto_tac)
+
+  also have "... = `($wait \<and> \<not> ok \<and> ($tr \<le> $tr\<acute>)) \<or> (ok' \<and> $wait \<and> II\<^bsub>REL_VAR - {okay\<down>, okay\<down>\<acute>}\<^esub>) \<or> (\<not>$wait \<and> P \<and> ( ok \<and> ($tr\<acute> =$tr) \<Rightarrow> $wait\<acute>))`" 
+    sorry
+
+  also have "... = `R3(P \<and> ( ok \<and> ($tr\<acute> =$tr) \<Rightarrow> $wait\<acute>))`" 
+    by(simp add: R3_def CondR_def SkipREA_def, utp_pred_auto_tac)
+
+  finally show ?thesis by(simp add:ACP1_def)
+qed
+
+lemma ACP1_OrP:
+  "`ACP1(P \<or> Q)` = `ACP1(P) \<or> ACP1(Q)`"
+  by (utp_pred_auto_tac)
+
+lemma ACP1_AndP:
+  "`ACP1(P \<and> Q)` = `ACP1(P) \<and> ACP1(Q)`"
+  by (utp_pred_auto_tac)
+
+lemma ACP1_CondR:
+  "`ACP1(P \<lhd> b \<rhd> Q)` = `ACP1(P) \<lhd> ACP1(b) \<rhd> ACP1(Q)`"
+  by (utp_pred_auto_tac)
+
+subsection {* \<delta> laws *}
+
+lemma R1_\<delta> : "`R1(\<delta>)` = `\<delta>`"
+proof -
+  have "`R1(\<delta>)`  = `(II\<^bsub>rea\<^esub> \<and> ($tr \<le> $tr\<acute>)) \<lhd> $wait \<rhd> ($tr =$tr\<acute> \<and> $wait\<acute> \<and> ($tr \<le> $tr\<acute>))`" 
+    by (simp add:\<delta>_def, utp_pred_auto_tac)
+  also have "... = `R1(II\<^bsub>rea\<^esub>) \<lhd> $wait \<rhd> ($tr\<acute> =$tr \<and> $wait\<acute> )`" 
+    by (utp_pred_auto_tac)
+  finally show ?thesis 
+    by (metis SkipREA_is_R1 R3_def \<delta>_def)
+qed
+
+lemma R2_\<delta> : "`R2(\<delta>)` = `\<delta>`" 
+proof -
+  have "`R2(\<delta>)`= `R3(R2($tr\<acute> = $tr) \<and> $wait\<acute>)`"
+    by (simp add:\<delta>_def R2_R3_commute, simp add:R2_def R1_def R2s_def usubst typing closure defined, utp_pred_auto_tac)
+  also have "... = `R3(($tr\<acute> = $tr) \<and> $wait\<acute>)`"
+    proof -
+    have "`R2($tr\<acute> = $tr)` = `($tr\<acute> = $tr)`" by (metis tr_conserved_is_R2)
+    thus ?thesis by metis
+    qed
+  finally show ?thesis by (simp add:\<delta>_def) 
+qed
+
+lemma R3_\<delta>: "`R3(\<delta>)` = `\<delta>`" 
+  by (simp add: \<delta>_def R3_idempotent)
+
+lemma ACP1_\<delta>: "ACP1(\<delta>) = \<delta>" 
+  by (simp add:is_healthy_def \<delta>_def ACP1_R3_commute, simp add:ACP1_def, utp_pred_auto_tac)
+
+lemma \<delta>_form: "\<delta> = `(\<not> ok \<and> $wait \<and> ($tr \<le> $tr\<acute>)) \<or> (ok \<and> $wait \<and> II) \<or> (\<not>$wait \<and> ($tr\<acute> = $tr) \<and> $wait\<acute>)`"
+  by(simp add: \<delta>_def R3_form) 
+
+subsection {* doA laws *}
+
+lemma doA_is_R1: "`R1(do\<A>(a))` = `do\<A>(a)`"
+  by (simp add:doA_def \<Phi>_def RH_def R1_idempotent)
+
+lemma doA_is_R2: "`R2(do\<A>(a))` = `do\<A>(a)`"
+  by (simp add:doA_def \<Phi>_def RH_def R1_R2_commute R2_idempotent)
+
+lemma doA_is_R3: "`R3(do\<A>(a))` = `do\<A>(a)`"
+  by (simp add:doA_def \<Phi>_def RH_def R2_R3_commute R1_R3_commute R3_idempotent)
+
+lemma doA_is_ACP1: "`do\<A>(a)` is ACP1" 
+proof -
+  have "`ACP1(B \<and>( a \<notin> $ref\<acute> \<lhd> $wait\<acute> \<rhd> ($tr^\<langle>a\<rangle> =$tr\<acute>)))` = `(B \<and>( a \<notin> $ref\<acute> \<lhd> $wait\<acute> \<rhd> ($tr^\<langle>a\<rangle> =$tr\<acute>)))`" 
+    by (simp add:ACP1_def CondR_def, utp_pred_auto_tac)
+  moreover have "`ACP1(do\<A>(a))` = `RH(ACP1(B \<and>( a \<notin> $ref\<acute> \<lhd> $wait\<acute> \<rhd> ($tr^\<langle>a\<rangle> =$tr\<acute>))))`" 
+    by (simp add:doA_def \<Phi>_def RH_def ACP1_R1_commute ACP1_R2_commute ACP1_R3_commute)
+  ultimately show ?thesis by(simp add:is_healthy_def doA_def \<Phi>_def)
+qed
+
+lemma B_form: "B = `R1($wait\<acute> \<or> ($tr < $tr\<acute>))`"
+  apply (utp_pred_auto_tac)
+  apply (metis prefixI)
+done
+
+lemma doA_form: 
+  assumes "TR \<sharp> a"
+  shows "`do\<A>(a)` = `R3(((a \<notin> $ref\<acute>) \<and> ($tr \<le> $tr\<acute>)) \<lhd> $wait\<acute> \<rhd> ($tr ^ \<langle>a\<rangle> = $tr\<acute>))`"
+proof -
+  have "`do\<A>(a)` = `RH(B \<and> ((a \<notin> $ref\<acute>) \<lhd> $wait\<acute> \<rhd> ($tr ^ \<langle>a\<rangle> = $tr\<acute>)))`" 
+    by (simp add: doA_def \<Phi>_def)
+
+  also have "... = `RH(((a \<notin> $ref\<acute>) \<and> ($tr \<le> $tr\<acute>)) \<lhd> $wait\<acute> \<rhd> (($tr ^ \<langle>a\<rangle> = $tr\<acute>) \<and> ($tr < $tr\<acute>)))`" 
+    proof -
+      have 1: "`($tr \<le> $tr\<acute>)` = `($tr < $tr\<acute>) \<or> ($tr\<acute> =  $tr)`"
+        by(utp_pred_auto_tac)
+      have 2: "`B \<and> $wait\<acute>` = `($tr \<le> $tr\<acute>) \<and> $wait\<acute>`"
+        apply(simp add:B_def "1")
+        apply(utp_pred_auto_tac)
+        done
+      have 3: "`B \<and> \<not>$wait\<acute>` = `($tr < $tr\<acute>) \<and> \<not>$wait\<acute>`"
+        apply(simp add:B_def)
+        apply(utp_pred_auto_tac)
+        done
+      have "`B \<and> ((a \<notin> $ref\<acute>) \<lhd> $wait\<acute> \<rhd> ($tr ^ \<langle>a\<rangle> = $tr\<acute>))` = `(B \<and> $wait\<acute> \<and> (a \<notin> $ref\<acute>)) \<or> (B \<and> \<not>$wait\<acute> \<and> ($tr ^ \<langle>a\<rangle> = $tr\<acute>))`"
+        apply(simp add:CondR_def)
+        apply(utp_pred_auto_tac)
+        done
+      also have "... = `(($tr \<le> $tr\<acute>) \<and> $wait\<acute> \<and> (a \<notin> $ref\<acute>)) \<or> (($tr < $tr\<acute>) \<and> \<not>$wait\<acute> \<and> ($tr ^ \<langle>a\<rangle> = $tr\<acute>))`"
+        by (smt "2" "3" AndP_assoc)
+      also have "... = `(($tr \<le> $tr\<acute>) \<and> (a \<notin> $ref\<acute>)) \<lhd> $wait\<acute> \<rhd> (($tr < $tr\<acute>) \<and> ($tr ^ \<langle>a\<rangle> = $tr\<acute>))`"
+        apply(simp add:CondR_def)
+        apply(utp_pred_auto_tac)
+        done
+      finally show ?thesis
+        by (metis AndP_comm)
+    qed
+  also have "... = `R3(R1(R2s(((a \<notin> $ref\<acute>) \<and> ($tr \<le> $tr\<acute>)) \<lhd> $wait\<acute> \<rhd> (($tr ^ \<langle>a\<rangle> = $tr\<acute>) \<and> ($tr < $tr\<acute>)))))`" 
+    by (simp add:RH_def R2_R3_commute R1_R3_commute, simp add:R2_def R1_idempotent)
+
+  also from assms have "... = `R3(R1((a \<notin> $ref\<acute>) \<lhd> $wait\<acute> \<rhd> (\<langle>a\<rangle> = ($tr\<acute> - $tr))))`"
+  proof -
+    have "`(($tr ^ \<langle>a\<rangle> = $tr\<acute>) \<and> ($tr < $tr\<acute>))` = `($tr ^ \<langle>a\<rangle> = $tr\<acute>)`"
+      apply (utp_pred_auto_tac)
+      apply (metis prefixI')
+    done
+
+    with assms show ?thesis
+      apply (simp)
+      apply (subgoal_tac "{tr\<down>} \<sharp> a")
+      apply (subgoal_tac "{tr\<down>\<acute>} \<sharp> a")
+      apply (simp add:R2s_def usubst typing defined closure unrest)
+      apply (auto intro:UNREST_PEXPR_subset)
+    done
+  qed
+
+  also have "... = `R3(R1((a \<notin> $ref\<acute>) \<lhd> $wait\<acute> \<rhd> ((\<langle>a\<rangle> = ($tr\<acute> - $tr)) \<and> ($tr \<le> $tr\<acute>))))`"
+    by (smt R1_CondR R1_def R1_idempotent)
+
+  also from assms have "... = `R3(R1((a \<notin> $ref\<acute>) \<lhd> $wait\<acute> \<rhd> ($tr ^ \<langle>a\<rangle> = $tr\<acute>)))`"
+  proof -
+    have "`\<langle>a\<rangle> = ($tr\<acute> - $tr) \<and> ($tr \<le> $tr\<acute>)` = `($tr ^ \<langle>a\<rangle>) = $tr\<acute> \<and> ($tr \<le> $tr\<acute>)`"
+      apply (utp_pred_tac)
+      apply (rule)
+      apply (subgoal_tac "set (drop (length (DestList (\<langle>b\<rangle>\<^sub>b tr\<down>))) (DestList (\<langle>b\<rangle>\<^sub>b tr\<down>\<acute>))) \<subseteq> dcarrier (EventType :: 'a UTYPE)")
+      apply (simp add:typing defined closure)
+      apply (smt drop_Cons' drop_all drop_append prefixeq_drop self_append_conv2)
+      apply (rule subset_trans, rule set_drop_subset, rule DestList_tr'_dcarrier)
+    done
+
+    thus ?thesis
+      by (metis tr_prefix_app)
+  qed
+
+  also have "... = `R3(((a \<notin> $ref\<acute>) \<and> ($tr \<le> $tr\<acute>)) \<lhd> $wait\<acute> \<rhd> (($tr ^ \<langle>a\<rangle> = $tr\<acute>) \<and> ($tr \<le> $tr\<acute>)))`" 
+    by (utp_pred_auto_tac)
+
+  finally show ?thesis
+    by (metis tr_prefix_app)
+
+qed
+
+subsection {*alternative laws *}
+
+lemma alternative_is_R1 :
+  assumes "P is R1" "Q is R1"
+  shows "P +\<^bsub>ACP\<^esub> Q is R1"
+  using assms
+  by (simp add:alternative_def is_healthy_def R1_CondR R1_AndP R1_OrP)
+
+lemma alternative_is_R2 :
+  assumes "P is R2" "Q is R2"
+  shows "(P +\<^bsub>ACP\<^esub> Q) is R2"
+proof -
+  have "R2 (P +\<^bsub>ACP\<^esub> Q) =  `R2(P \<and> Q) \<lhd> R2(\<delta>) \<rhd> R2(P \<or> Q)`" 
+    by (simp add:alternative_def R2_CondR_alt)
+
+  also have "... = `(R2(P) \<and> R2(Q)) \<lhd> \<delta> \<rhd> (R2(P) \<or> R2(Q))`" 
+    by (simp add: R2_\<delta> R2_AndP R2_OrP)
+
+  also from assms 
+  have "... = `(P \<and> Q) \<lhd> \<delta> \<rhd> (P \<or> Q)`" 
+    by (simp add:is_healthy_def)
+
+  also have "... = P +\<^bsub>ACP\<^esub> Q"
+    by (simp add:alternative_def)
+
+  finally show ?thesis 
+    by (simp add:is_healthy_def)
+qed
+
+lemma alternative_is_R3 : 
+  assumes "P is R3" "Q is R3"
+  shows "(P +\<^bsub>ACP\<^esub> Q) is R3"
+  using assms
+  by (simp add:alternative_def is_healthy_def R3_CondR R3_AndP R3_OrP R3_\<delta>)
+
+lemma alternative_is_ACP1 :
+  assumes "P is ACP1" "Q is ACP1"
+  shows "(P +\<^bsub>ACP\<^esub> Q) is ACP1"
+using assms
+  by (simp add:is_healthy_def alternative_def ACP1_CondR ACP1_OrP ACP1_AndP ACP1_\<delta>)
+
+subsection {*ACP laws *}
+
+lemma L1 :
+  assumes "P is ACP1" "P is RH" "P \<in> WF_RELATION"
+  shows "\<delta> ; P = \<delta>"  
+proof -
+  have 1: "`\<delta> ; P` is R3"
+    apply(subst R3_SemiR_closure)
+    apply (metis \<delta>_rel_closure)
+    apply (metis assms(3))
+    apply (metis Healthy_intro R3_\<delta>)
+    apply (metis RH_is_R3 assms(2))
+    apply (metis RH_is_R1 assms(2))
+    apply (simp)
+    done
+  have 2: "`\<not>$wait \<and> \<delta>` = `\<not>$wait \<and> ($tr\<acute> = $tr) \<and> $wait\<acute>`" 
+    by(utp_pred_auto_tac)
+  have "`\<not>$wait \<and> \<delta>;P` = `(\<not>$wait \<and> \<delta>) ; P`"
+    apply(subst SemiR_AndP_left_precond)
+    apply (metis \<delta>_rel_closure)
+    apply (metis assms(3))
+    apply (utp_pred_auto_tac)
+    apply (simp)
+    done
+  also have "... = `(\<not>$wait \<and> ($tr\<acute> = $tr) \<and> $wait\<acute>) ; P`" 
+    by(subst 2,simp)
+  also have "... = `(\<not>$wait \<and> ($tr\<acute> = $tr)) ; ($wait \<and> P)`"
+    apply(subst SemiR_AndP_right_precond)
+    apply(subst AndP_rel_closure)
+    apply(utp_pred_auto_tac)
+    apply(metis tr_eq_rel_closure)
+    apply(simp_all)
+    apply(simp add: assms (3))
+    apply(utp_pred_auto_tac)
+    apply(simp add: urename closure typing defined )
+    apply (metis (hide_lams, mono_tags) AndP_assoc)
+done
+ also have "... = `(\<not>$wait \<and> ($tr\<acute> = $tr)) ; ($wait \<and> R3(P))`"
+    by(metis assms(2) RH_is_R3 is_healthy_def)
+  also have "... = `(\<not>$wait \<and> ($tr\<acute> = $tr)) ; ($wait \<and> II\<^bsub>rea\<^esub>)`"
+    by (metis AndP_comm R3_wait)
+  also have "... = `(\<not>$wait \<and> ($tr\<acute> = $tr) \<and> $wait\<acute>) ; II\<^bsub>rea\<^esub>`"
+    apply(subst SemiR_AndP_right_precond)
+    apply(subst AndP_rel_closure)
+    apply(utp_pred_auto_tac)
+    apply(metis tr_eq_rel_closure)
+    apply(simp_all)
+    apply(metis SkipREA_rel_closure)
+    apply(utp_pred_auto_tac)
+    apply(simp add: urename closure typing defined )
+by (metis (hide_lams, mono_tags) AndP_assoc)
+  also have "... = `\<not>$wait \<and> (($tr\<acute> = $tr) \<and> $wait\<acute>) ; II\<^bsub>rea\<^esub>`"
+    apply(subst SemiR_AndP_left_precond)
+    apply(subst AndP_rel_closure)
+    apply(metis tr_eq_rel_closure)
+    apply(utp_pred_auto_tac)
+    apply(simp_all)
+    apply(metis SkipREA_rel_closure)
+    apply(utp_pred_auto_tac)
+    done
+  finally have 3: "`\<not>$wait \<and> \<delta>;P` = `\<not>$wait \<and> (($tr\<acute> = $tr) \<and> $wait\<acute>) ; II\<^bsub>rea\<^esub>`"
+    ..
+  have "`(($tr\<acute> = $tr) \<and> $wait\<acute>) ; II\<^bsub>rea\<^esub>` = `
+        (($tr\<acute> = $tr) \<and> $wait\<acute>) ; (ok \<and> II\<^bsub>REL_VAR\<^esub>) \<or>
+        (($tr\<acute> = $tr) \<and> $wait\<acute>) ; (\<not>ok \<and> ($tr \<le> $tr\<acute>))`" 
+    by(simp add:SkipREA_CondR_SkipR CondR_def SemiR_OrP_distl SkipR_as_SkipRA)
+  also have "... = `
+        (($tr\<acute> = $tr) \<and> $wait\<acute> \<and> ok') ; II\<^bsub>REL_VAR\<^esub> \<or>
+        (($tr\<acute> = $tr) \<and> $wait\<acute> \<and> \<not>ok') ; ($tr \<le> $tr\<acute>)`"
+    apply(subst SemiR_AndP_right_precond)
+    apply(subst AndP_rel_closure)
+    apply(metis tr_eq_rel_closure)
+    apply(utp_pred_auto_tac)
+    apply(simp_all)
+    apply (metis SkipR_as_SkipRA SkipR_closure)
+    apply(utp_pred_auto_tac)
+    apply(subst SemiR_AndP_right_precond)
+    apply(subst AndP_rel_closure)
+    apply(metis tr_eq_rel_closure)
+    apply(utp_pred_auto_tac)
+    apply(simp_all)
+    apply (smt R1_def R1_rel_closure TrueP_rel_closure utp_pred_simps(6))
+    apply(utp_pred_auto_tac)    
+    apply(simp add: urename closure typing defined )
+    by (metis (hide_lams, no_types) AndP_assoc AndP_comm SemiR_assoc SkipR_as_SkipRA demorgan3 utp_pred_simps(15))
+  also have "... = `
+        (($tr\<acute> = $tr) \<and> $wait\<acute> \<and> ok')  \<or>
+        (($tr\<acute> = $tr) \<and> $wait\<acute> \<and> \<not>ok') ; ($tr \<le> $tr\<acute>)`"
+    apply(subst SkipRA_right_unit)
+    apply(subst AndP_rel_closure)
+    apply (metis tr_eq_rel_closure)
+    apply(utp_pred_auto_tac)
+    apply(simp_all add:closure unrest typing)
+    done
+  also have "... = `
+        (($tr\<acute> = $tr) \<and> $wait\<acute> \<and> ok')  \<or>
+        ($tr\<acute> = $tr) ; ((\<not>ok \<and> $wait) \<and> ($tr \<le> $tr\<acute>))`"
+    apply(subst SemiR_AndP_right_precond)
+    apply(simp_all add:closure typing WF_RELATION_UNREST defined unrest urename AndP_comm)
+    done
+  also have "... = `(($tr\<acute> = $tr) \<and> $wait\<acute> \<and> ok')  \<or> 
+                      ($tr\<acute> = $tr) ; ($tr \<le> $tr\<acute>)`"
+    apply(subst SemiR_remove_middle_unrest1[of "`($tr \<acute>=$tr)`" "`($tr \<le> $tr \<acute>)`" "{wait \<down>,okay \<down>}" "`\<not>ok \<and> $wait`"])
+    apply(simp_all add:closure unrest typing defined WF_RELATION_UNREST)
+    apply(utp_pred_auto_tac)
+    apply(rule_tac x="\<B>(okay\<down> :=\<^sub>b FalseV, wait\<down> :=\<^sub>b TrueV)" in exI)
+    apply(simp add:typing defined)
+  done
+  also have "... = `(($tr\<acute> = $tr) \<and> $wait\<acute> \<and> ok')  \<or> ($tr \<le> $tr\<acute>)`"
+    by (metis tr_eq_tr_leq)
+  finally have 4: "`(($tr\<acute> = $tr) \<and> $wait\<acute>) ; II\<^bsub>rea\<^esub>` = `($tr \<le> $tr\<acute>)`"
+    by(utp_pred_auto_tac)
+  have "`\<delta> ; P` = `R3(\<delta> ; P)`"
+    by(metis "1" is_healthy_def)
+  also have "... = `(\<not>ok \<and> $wait \<and> ($tr \<le> $tr\<acute>)) \<or> (ok \<and> $wait \<and> II) \<or> (\<not>$wait \<and> \<delta> ; P)`"
+    by (simp add:R3_form)
+  also have "... = `(\<not>ok \<and> $wait \<and> ($tr \<le> $tr\<acute>)) \<or> (ok \<and> $wait \<and> II) \<or> (\<not>$wait \<and> (($tr\<acute> = $tr) \<and> $wait\<acute>) ; II\<^bsub>rea\<^esub>)`"
+    by (simp add:"3")
+  also have "... = `(\<not>ok \<and> $wait \<and> ($tr \<le> $tr\<acute>)) \<or> (ok \<and> $wait \<and> II) \<or> (\<not>$wait \<and> ($tr \<le> $tr\<acute>))`"
+    by (metis "4")
+  also have "... = RH true"
+    by(simp add:RH_def R2_R3_commute R1_R3_commute, simp add:R2_def R1_idempotent R2s_def usubst typing closure defined R1_def R3_form)
+  finally have 5: " \<delta> ; P = RH true " ..
+oops
+
+lemma L2 : "P +\<^bsub>ACP\<^esub> P = P" 
+  by(simp add: alternative_def, utp_pred_auto_tac)
+
+lemma L3 : "P +\<^bsub>ACP\<^esub> Q = Q +\<^bsub>ACP\<^esub> P"
+  by (metis AndP_comm OrP_comm alternative_def) 
+
+lemma L4 : "(P +\<^bsub>ACP\<^esub> Q) +\<^bsub>ACP\<^esub> R = P +\<^bsub>ACP\<^esub> (Q +\<^bsub>ACP\<^esub> R)" 
+  proof -
+  have "(P +\<^bsub>ACP\<^esub> Q) +\<^bsub>ACP\<^esub> R =`(P \<and> Q \<and> R)  \<lhd> \<delta> \<rhd>  (P \<or> Q \<or> R)`"
+    proof-
+    have 1: "`(P + Q) \<and>  \<delta>` = `P \<and> Q \<and> \<delta>`" 
+      apply(simp add:alternative_def CondR_def) 
+      apply (metis AndP_assoc AndP_comm CondR_def CondR_true_cond)
+      done
+    have 2: "`(P + Q) \<and>  \<not>\<delta>` = `(P \<or> Q) \<and> \<not>\<delta>`" 
+      apply(simp add:alternative_def CondR_def) 
+      apply (metis AndP_comm CondR_def CondR_false_cond)
+      done
+    have "(P +\<^bsub>ACP\<^esub> Q) +\<^bsub>ACP\<^esub> R = `((P + Q) \<and> R) \<lhd> \<delta> \<rhd> ((P + Q) \<or> R)` "
+     by(simp add: alternative_def)
+     also have "... = `((\<delta> \<and> R \<and> (P + Q)) \<or> (\<not> \<delta> \<and> (P + Q)) \<or> (R \<and> \<not> \<delta>))` "
+    by(simp add:CondR_def AndP_OrP_distl AndP_comm)
+    also have "... = `((\<delta> \<and> R \<and> (P \<and> Q)) \<or> (\<not> \<delta> \<and> (P \<or> Q)) \<or> (R \<and> \<not> \<delta>))` "
+    by (smt "1" "2" AndP_assoc AndP_comm)
+    also have "... = `(\<delta> \<and> (R \<and> P \<and> Q)) \<or> (\<not> \<delta> \<and> (P \<or> Q \<or> R))` " 
+    by (smt AndP_OrP_distl AndP_comm OrP_assoc)
+    finally show ?thesis by (metis AndP_assoc AndP_comm CondR_def)
+  qed
+  moreover have "P +\<^bsub>ACP\<^esub> (Q +\<^bsub>ACP\<^esub> R) =`(P \<and> Q \<and> R)  \<lhd> \<delta> \<rhd>  (P \<or> Q \<or> R)`"
+    proof-
+    have 3: "`(Q + R) \<and>  \<delta>` = `Q \<and> R \<and> \<delta>`" 
+      apply(simp add:alternative_def CondR_def) 
+      apply (metis AndP_assoc AndP_comm CondR_def CondR_true_cond)
+      done
+    have 4: "`(Q + R) \<and>  \<not>\<delta>` = `(Q \<or> R) \<and> \<not>\<delta>`" 
+      apply(simp add:alternative_def CondR_def) 
+      apply (metis AndP_comm CondR_def CondR_false_cond)
+      done
+    have "P +\<^bsub>ACP\<^esub> (Q +\<^bsub>ACP\<^esub> R) = `(P \<and> (Q + R)) \<lhd> \<delta> \<rhd> (P \<or> (Q + R))` "
+     by(simp add: alternative_def)
+     also have "... = `((\<delta> \<and> P \<and> (Q + R)) \<or> (P \<and> \<not> \<delta>) \<or> (\<not> \<delta> \<and> (Q + R)) )` "
+    by(simp add:CondR_def AndP_OrP_distl AndP_comm)
+    also have "... = `((\<delta> \<and> P \<and> (Q \<and> R))  \<or> (P \<and> \<not> \<delta>) \<or> (\<not> \<delta> \<and> (Q \<or> R)))` "
+    by (smt "3" "4" AndP_assoc AndP_comm)
+    also have "... = `(\<delta> \<and> (P \<and> Q \<and> R)) \<or> (\<not> \<delta> \<and> (P \<or> Q \<or> R))` " 
+    by (smt AndP_OrP_distl AndP_comm OrP_assoc)
+    finally show ?thesis by (metis AndP_assoc AndP_comm CondR_def)
+  qed
+  ultimately show ?thesis ..
+qed
+
+lemma L5 : "\<delta> +\<^bsub>ACP\<^esub> Q = Q" 
+  by(simp add:alternative_def, utp_pred_auto_tac)
+
+lemma L6 : 
+  assumes "S is ACP1" "S is RH" "S \<in> WF_RELATION"
+  shows "(P +\<^bsub>ACP\<^esub> Q) ; S = (P;S) +\<^bsub>ACP\<^esub> (Q;S)"
+oops
+end
